tests/test.bpl
@@ -1,9 +1,9 @@
 // 
 // Translation of Viper program.
 // 
-// Date:         2021-04-09 17:41:45
+// Date:         2021-04-13 13:40:00
 // Tool:         carbon 1.0
-// Arguments: :  --z3Exe /usr/bin/z3 --boogieExe /bin/boogie/Binaries/boogie --translateOnly --print tests/test.bpl tests/test.vpr
+// Arguments: :  --z3Exe /usr/bin/z3 --boogieExe /bin/boogie/Binaries/boogie --print ../../clean/carbon/tests/test.bpl ../../clean/carbon/benchmarking/failed/0196.vpr
 // Dependencies:
 //   Boogie , located at /bin/boogie/Binaries/boogie.
 //   Z3 4.8.4 - 64 bit, located at /usr/bin/z3.
@@ -13,7 +13,7 @@
 // Preamble of State module.
 // ==================================================
 
-function  state(Heap: HeapType, Mask: MaskType, BMask: BMaskType): bool;
+function  state(Heap: HeapType, Mask: MaskType): bool;
 
 // ==================================================
 // Preamble of Heap module.
@@ -32,45 +32,45 @@ axiom (forall o: Ref, f: (Field NormalField Ref), Heap: HeapType ::
 );
 function  succHeap(Heap0: HeapType, Heap1: HeapType): bool;
 function  succHeapTrans(Heap0: HeapType, Heap1: HeapType): bool;
-function  IdenticalOnKnownLocations(Heap: HeapType, ExhaleHeap: HeapType, Mask: MaskType, BMask: BMaskType): bool;
+function  IdenticalOnKnownLocations(Heap: HeapType, ExhaleHeap: HeapType, Mask: MaskType): bool;
 function  IsPredicateField<A, B>(f_1: (Field A B)): bool;
 function  IsWandField<A, B>(f_1: (Field A B)): bool;
 function  getPredicateId<A, B>(f_1: (Field A B)): int;
 // Frame all locations with direct permissions
-axiom (forall <A, B> Heap: HeapType, ExhaleHeap: HeapType, Mask: MaskType, BMask: BMaskType, o: Ref, f_2: (Field A B) ::
-  { IdenticalOnKnownLocations(Heap, ExhaleHeap, Mask, BMask), ExhaleHeap[o, f_2] }
-  IdenticalOnKnownLocations(Heap, ExhaleHeap, Mask, BMask) ==> HasDirectPerm(Mask, BMask, o, f_2) ==> Heap[o, f_2] == ExhaleHeap[o, f_2]
+axiom (forall <A, B> Heap: HeapType, ExhaleHeap: HeapType, Mask: MaskType, o: Ref, f_2: (Field A B) ::
+  { IdenticalOnKnownLocations(Heap, ExhaleHeap, Mask), ExhaleHeap[o, f_2] }
+  IdenticalOnKnownLocations(Heap, ExhaleHeap, Mask) ==> HasDirectPerm(Mask, o, f_2) ==> Heap[o, f_2] == ExhaleHeap[o, f_2]
 );
 // Frame all predicate mask locations of predicates with direct permission
-axiom (forall <C> Heap: HeapType, ExhaleHeap: HeapType, Mask: MaskType, BMask: BMaskType, pm_f: (Field C FrameType) ::
-  { IdenticalOnKnownLocations(Heap, ExhaleHeap, Mask, BMask), IsPredicateField(pm_f), ExhaleHeap[null, PredicateMaskField(pm_f)] }
-  IdenticalOnKnownLocations(Heap, ExhaleHeap, Mask, BMask) ==> HasDirectPerm(Mask, BMask, null, pm_f) && IsPredicateField(pm_f) ==> Heap[null, PredicateMaskField(pm_f)] == ExhaleHeap[null, PredicateMaskField(pm_f)]
+axiom (forall <C> Heap: HeapType, ExhaleHeap: HeapType, Mask: MaskType, pm_f: (Field C FrameType) ::
+  { IdenticalOnKnownLocations(Heap, ExhaleHeap, Mask), IsPredicateField(pm_f), ExhaleHeap[null, PredicateMaskField(pm_f)] }
+  IdenticalOnKnownLocations(Heap, ExhaleHeap, Mask) ==> HasDirectPerm(Mask, null, pm_f) && IsPredicateField(pm_f) ==> Heap[null, PredicateMaskField(pm_f)] == ExhaleHeap[null, PredicateMaskField(pm_f)]
 );
 // Frame all locations with known folded permissions
-axiom (forall <C> Heap: HeapType, ExhaleHeap: HeapType, Mask: MaskType, BMask: BMaskType, pm_f: (Field C FrameType) ::
-  { IdenticalOnKnownLocations(Heap, ExhaleHeap, Mask, BMask), ExhaleHeap[null, pm_f], IsPredicateField(pm_f) }
-  IdenticalOnKnownLocations(Heap, ExhaleHeap, Mask, BMask) ==> HasDirectPerm(Mask, BMask, null, pm_f) && IsPredicateField(pm_f) ==> (forall <A, B> o2: Ref, f_2: (Field A B) ::
+axiom (forall <C> Heap: HeapType, ExhaleHeap: HeapType, Mask: MaskType, pm_f: (Field C FrameType) ::
+  { IdenticalOnKnownLocations(Heap, ExhaleHeap, Mask), ExhaleHeap[null, pm_f], IsPredicateField(pm_f) }
+  IdenticalOnKnownLocations(Heap, ExhaleHeap, Mask) ==> HasDirectPerm(Mask, null, pm_f) && IsPredicateField(pm_f) ==> (forall <A, B> o2: Ref, f_2: (Field A B) ::
     { ExhaleHeap[o2, f_2] }
     Heap[null, PredicateMaskField(pm_f)][o2, f_2] ==> Heap[o2, f_2] == ExhaleHeap[o2, f_2]
   )
 );
 // Frame all wand mask locations of wands with direct permission
-axiom (forall <C> Heap: HeapType, ExhaleHeap: HeapType, Mask: MaskType, BMask: BMaskType, pm_f: (Field C FrameType) ::
-  { IdenticalOnKnownLocations(Heap, ExhaleHeap, Mask, BMask), IsWandField(pm_f), ExhaleHeap[null, WandMaskField(pm_f)] }
-  IdenticalOnKnownLocations(Heap, ExhaleHeap, Mask, BMask) ==> HasDirectPerm(Mask, BMask, null, pm_f) && IsWandField(pm_f) ==> Heap[null, WandMaskField(pm_f)] == ExhaleHeap[null, WandMaskField(pm_f)]
+axiom (forall <C> Heap: HeapType, ExhaleHeap: HeapType, Mask: MaskType, pm_f: (Field C FrameType) ::
+  { IdenticalOnKnownLocations(Heap, ExhaleHeap, Mask), IsWandField(pm_f), ExhaleHeap[null, WandMaskField(pm_f)] }
+  IdenticalOnKnownLocations(Heap, ExhaleHeap, Mask) ==> HasDirectPerm(Mask, null, pm_f) && IsWandField(pm_f) ==> Heap[null, WandMaskField(pm_f)] == ExhaleHeap[null, WandMaskField(pm_f)]
 );
 // Frame all locations in the footprint of magic wands
-axiom (forall <C> Heap: HeapType, ExhaleHeap: HeapType, Mask: MaskType, BMask: BMaskType, pm_f: (Field C FrameType) ::
-  { IdenticalOnKnownLocations(Heap, ExhaleHeap, Mask, BMask), IsWandField(pm_f) }
-  IdenticalOnKnownLocations(Heap, ExhaleHeap, Mask, BMask) ==> HasDirectPerm(Mask, BMask, null, pm_f) && IsWandField(pm_f) ==> (forall <A, B> o2: Ref, f_2: (Field A B) ::
+axiom (forall <C> Heap: HeapType, ExhaleHeap: HeapType, Mask: MaskType, pm_f: (Field C FrameType) ::
+  { IdenticalOnKnownLocations(Heap, ExhaleHeap, Mask), IsWandField(pm_f) }
+  IdenticalOnKnownLocations(Heap, ExhaleHeap, Mask) ==> HasDirectPerm(Mask, null, pm_f) && IsWandField(pm_f) ==> (forall <A, B> o2: Ref, f_2: (Field A B) ::
     { ExhaleHeap[o2, f_2] }
     Heap[null, WandMaskField(pm_f)][o2, f_2] ==> Heap[o2, f_2] == ExhaleHeap[o2, f_2]
   )
 );
 // All previously-allocated references are still allocated
-axiom (forall Heap: HeapType, ExhaleHeap: HeapType, Mask: MaskType, BMask: BMaskType, o: Ref ::
-  { IdenticalOnKnownLocations(Heap, ExhaleHeap, Mask, BMask), ExhaleHeap[o, $allocated] }
-  IdenticalOnKnownLocations(Heap, ExhaleHeap, Mask, BMask) ==> Heap[o, $allocated] ==> ExhaleHeap[o, $allocated]
+axiom (forall Heap: HeapType, ExhaleHeap: HeapType, Mask: MaskType, o: Ref ::
+  { IdenticalOnKnownLocations(Heap, ExhaleHeap, Mask), ExhaleHeap[o, $allocated] }
+  IdenticalOnKnownLocations(Heap, ExhaleHeap, Mask) ==> Heap[o, $allocated] ==> ExhaleHeap[o, $allocated]
 );
 // Updated Heaps are Successor Heaps
 axiom (forall <A, B> Heap: HeapType, o: Ref, f_2: (Field A B), v: B ::
@@ -78,9 +78,9 @@ axiom (forall <A, B> Heap: HeapType, o: Ref, f_2: (Field A B), v: B ::
   succHeap(Heap, Heap[o, f_2:=v])
 );
 // IdenticalOnKnownLocations Heaps are Successor Heaps
-axiom (forall Heap: HeapType, ExhaleHeap: HeapType, Mask: MaskType, BMask: BMaskType ::
-  { IdenticalOnKnownLocations(Heap, ExhaleHeap, Mask, BMask) }
-  IdenticalOnKnownLocations(Heap, ExhaleHeap, Mask, BMask) ==> succHeap(Heap, ExhaleHeap)
+axiom (forall Heap: HeapType, ExhaleHeap: HeapType, Mask: MaskType ::
+  { IdenticalOnKnownLocations(Heap, ExhaleHeap, Mask) }
+  IdenticalOnKnownLocations(Heap, ExhaleHeap, Mask) ==> succHeap(Heap, ExhaleHeap)
 );
 // Successor Heaps are Transitive Successor Heaps
 axiom (forall Heap0: HeapType, Heap1: HeapType ::
@@ -100,17 +100,10 @@ axiom (forall Heap0: HeapType, Heap1: HeapType, Heap2: HeapType ::
 type Perm = real;
 type MaskType = <A, B> [Ref, Field A B]Perm;
 var Mask: MaskType;
-type BMaskType = <A, B> [Ref, Field A B]bool;
-var BMask: BMaskType;
 const ZeroMask: MaskType;
 axiom (forall <A, B> o_1: Ref, f_3: (Field A B) ::
   { ZeroMask[o_1, f_3] }
   ZeroMask[o_1, f_3] == NoPerm
-);
-const ZeroBMask: BMaskType;
-axiom (forall <A, B> o_1: Ref, f_3: (Field A B) ::
-  { ZeroBMask[o_1, f_3] }
-  !ZeroBMask[o_1, f_3]
 );
 type PMaskType = <A, B> [Ref, Field A B]bool;
 const ZeroPMask: PMaskType;
@@ -125,19 +118,19 @@ axiom NoPerm == 0.000000000;
 const FullPerm: Perm;
 axiom FullPerm == 1.000000000;
 function  Perm(a: real, b: real): Perm;
-function  GoodMask(Mask: MaskType, BMask: BMaskType): bool;
-axiom (forall Heap: HeapType, Mask: MaskType, BMask: BMaskType ::
-  { state(Heap, Mask, BMask) }
-  state(Heap, Mask, BMask) ==> GoodMask(Mask, BMask)
+function  GoodMask(Mask: MaskType): bool;
+axiom (forall Heap: HeapType, Mask: MaskType ::
+  { state(Heap, Mask) }
+  state(Heap, Mask) ==> GoodMask(Mask)
 );
-axiom (forall <A, B> Mask: MaskType, BMask: BMaskType, o_1: Ref, f_3: (Field A B) ::
-  { GoodMask(Mask, BMask), Mask[o_1, f_3] }
-  GoodMask(Mask, BMask) ==> Mask[o_1, f_3] >= NoPerm && ((GoodMask(Mask, BMask) && !IsPredicateField(f_3)) && !IsWandField(f_3) ==> Mask[o_1, f_3] <= FullPerm && (Mask[o_1, f_3] == FullPerm ==> !BMask[o_1, f_3]))
+axiom (forall <A, B> Mask: MaskType, o_1: Ref, f_3: (Field A B) ::
+  { GoodMask(Mask), Mask[o_1, f_3] }
+  GoodMask(Mask) ==> Mask[o_1, f_3] >= NoPerm && ((GoodMask(Mask) && !IsPredicateField(f_3)) && !IsWandField(f_3) ==> Mask[o_1, f_3] <= FullPerm)
 );
-function  HasDirectPerm<A, B>(Mask: MaskType, BMask: BMaskType, o_1: Ref, f_3: (Field A B)): bool;
-axiom (forall <A, B> Mask: MaskType, BMask: BMaskType, o_1: Ref, f_3: (Field A B) ::
-  { HasDirectPerm(Mask, BMask, o_1, f_3) }
-  HasDirectPerm(Mask, BMask, o_1, f_3) <==> Mask[o_1, f_3] > NoPerm || BMask[o_1, f_3]
+function  HasDirectPerm<A, B>(Mask: MaskType, o_1: Ref, f_3: (Field A B)): bool;
+axiom (forall <A, B> Mask: MaskType, o_1: Ref, f_3: (Field A B) ::
+  { HasDirectPerm(Mask, o_1, f_3) }
+  HasDirectPerm(Mask, o_1, f_3) <==> Mask[o_1, f_3] > NoPerm
 );
 function  sumMask(ResultMask: MaskType, SummandMask1: MaskType, SummandMask2: MaskType): bool;
 axiom (forall <A, B> ResultMask: MaskType, SummandMask1: MaskType, SummandMask2: MaskType, o_1: Ref, f_3: (Field A B) ::
@@ -148,25 +141,99 @@ axiom (forall <A, B> ResultMask: MaskType, SummandMask1: MaskType, SummandMask2:
 // Function for trigger used in checks which are never triggered
 // ==================================================
 
-function  neverTriggered1(r_1: Ref): bool;
-function  neverTriggered2(r_3: Ref): bool;
+function  neverTriggered1(e: Ref): bool;
+function  neverTriggered2(e_2: Ref): bool;
+function  neverTriggered3(e_3: Ref): bool;
+function  neverTriggered4(e: Ref): bool;
+function  neverTriggered5(e_2: Ref): bool;
+function  neverTriggered6(e_3: Ref): bool;
+function  neverTriggered7(e: Ref): bool;
+function  neverTriggered8(e_2: Ref): bool;
+function  neverTriggered9(e_3: Ref): bool;
+function  neverTriggered10(e: Ref): bool;
+function  neverTriggered11(e_2: Ref): bool;
+function  neverTriggered12(e_3: Ref): bool;
+function  neverTriggered13(e: Ref): bool;
+function  neverTriggered14(e_1: Ref): bool;
+function  neverTriggered15(e_3: Ref): bool;
+function  neverTriggered16(e: Ref): bool;
+function  neverTriggered17(e_1: Ref): bool;
+function  neverTriggered18(e_3: Ref): bool;
+function  neverTriggered19(e: Ref): bool;
+function  neverTriggered20(e_1: Ref): bool;
+function  neverTriggered21(e_3: Ref): bool;
+function  neverTriggered22(e: Ref): bool;
+function  neverTriggered23(e_1: Ref): bool;
+function  neverTriggered24(e_3: Ref): bool;
 // ==================================================
 // Functions used as inverse of receiver expressions in quantified permissions during inhale and exhale
 // ==================================================
 
-function  invRecv1(recv: Ref): Ref;
-function  invRecv2(recv: Ref): Ref;
+function  invRecv1(r_1_1: Ref): Ref;
+function  invRecv2(r_2_1: Ref): Ref;
+function  invRecv3(r_3_1: Ref): Ref;
+function  invRecv4(r_1_1: Ref): Ref;
+function  invRecv5(r_2_1: Ref): Ref;
+function  invRecv6(r_3_1: Ref): Ref;
+function  invRecv7(r_1_1: Ref): Ref;
+function  invRecv8(r_2_1: Ref): Ref;
+function  invRecv9(r_3_1: Ref): Ref;
+function  invRecv10(r_1_1: Ref): Ref;
+function  invRecv11(r_2_1: Ref): Ref;
+function  invRecv12(r_3_1: Ref): Ref;
+function  invRecv13(recv: Ref): Ref;
+function  invRecv14(recv: Ref): Ref;
+function  invRecv15(recv: Ref): Ref;
+function  invRecv16(recv: Ref): Ref;
+function  invRecv17(recv: Ref): Ref;
+function  invRecv18(recv: Ref): Ref;
+function  invRecv19(recv: Ref): Ref;
+function  invRecv20(recv: Ref): Ref;
+function  invRecv21(recv: Ref): Ref;
+function  invRecv22(recv: Ref): Ref;
+function  invRecv23(recv: Ref): Ref;
+function  invRecv24(recv: Ref): Ref;
 // ==================================================
 // Functions used to represent the range of the projection of each QP instance onto its receiver expressions for quantified permissions during inhale and exhale
 // ==================================================
 
-function  qpRange1(recv: Ref): bool;
-function  qpRange2(recv: Ref): bool;
+function  qpRange1(r_1_1: Ref): bool;
+function  qpRange2(r_2_1: Ref): bool;
+function  qpRange3(r_3_1: Ref): bool;
+function  qpRange4(r_1_1: Ref): bool;
+function  qpRange5(r_2_1: Ref): bool;
+function  qpRange6(r_3_1: Ref): bool;
+function  qpRange7(r_1_1: Ref): bool;
+function  qpRange8(r_2_1: Ref): bool;
+function  qpRange9(r_3_1: Ref): bool;
+function  qpRange10(r_1_1: Ref): bool;
+function  qpRange11(r_2_1: Ref): bool;
+function  qpRange12(r_3_1: Ref): bool;
+function  qpRange13(recv: Ref): bool;
+function  qpRange14(recv: Ref): bool;
+function  qpRange15(recv: Ref): bool;
+function  qpRange16(recv: Ref): bool;
+function  qpRange17(recv: Ref): bool;
+function  qpRange18(recv: Ref): bool;
+function  qpRange19(recv: Ref): bool;
+function  qpRange20(recv: Ref): bool;
+function  qpRange21(recv: Ref): bool;
+function  qpRange22(recv: Ref): bool;
+function  qpRange23(recv: Ref): bool;
+function  qpRange24(recv: Ref): bool;
 
 // ==================================================
 // Preamble of Function and predicate module.
 // ==================================================
 
+// Function heights (higher height means its body is available earlier):
+// - height 5: refs
+// - height 4: testerFull
+// - height 3: get
+// - height 2: testerfieldFull
+// - height 1: tester
+// - height 0: testerfield
+const AssumeFunctionsAbove: int;
 // Declarations for function framing
 type FrameType;
 const EmptyFrame: FrameType;
@@ -390,153 +457,2640 @@ axiom (forall<T> a: MultiSet T, b: MultiSet T :: { MultiSet#Disjoint(a,b) }
 // Translation of all fields
 // ==================================================
 
-const unique f_6: Field NormalField int;
-axiom !IsPredicateField(f_6);
-axiom !IsWandField(f_6);
+const unique q_1: Field NormalField Ref;
+axiom !IsPredicateField(q_1);
+axiom !IsWandField(q_1);
 
 // ==================================================
-// Translation of method main
+// Translation of function refs
 // ==================================================
 
-procedure main(s: (Set Ref)) returns ()
-  modifies Heap, Mask, BMask;
+// Uninterpreted function definitions
+function  refs(Heap: HeapType, r_1: Ref): Set Ref;
+function  refs'(Heap: HeapType, r_1: Ref): Set Ref;
+axiom (forall Heap: HeapType, r_1: Ref ::
+  { refs(Heap, r_1) }
+  refs(Heap, r_1) == refs'(Heap, r_1) && dummyFunction(refs#triggerStateless(r_1))
+);
+axiom (forall Heap: HeapType, r_1: Ref ::
+  { refs'(Heap, r_1) }
+  dummyFunction(refs#triggerStateless(r_1))
+);
+
+// Framing axioms
+function  refs#frame(frame: FrameType, r_1: Ref): Set Ref;
+axiom (forall Heap: HeapType, Mask: MaskType, r_1: Ref ::
+  { state(Heap, Mask), refs'(Heap, r_1) }
+  state(Heap, Mask) ==> refs'(Heap, r_1) == refs#frame(EmptyFrame, r_1)
+);
+
+// Trigger function (controlling recursive postconditions)
+function  refs#trigger(frame: FrameType, r_1: Ref): bool;
+
+// State-independent trigger function
+function  refs#triggerStateless(r_1: Ref): Set Ref;
+
+// Check contract well-formedness and postcondition
+procedure refs#definedness(r_1: Ref) returns (Result: (Set Ref))
+  modifies Heap, Mask;
 {
-  var x: Ref;
-  var y: Ref;
+  
+  // -- Initializing the state
+    Mask := ZeroMask;
+    assume state(Heap, Mask);
+    assume Heap[r_1, $allocated];
+    assume AssumeFunctionsAbove == 5;
+  
+  // -- Initializing the old state
+    assume Heap == old(Heap);
+    assume Mask == old(Mask);
+}
+
+// ==================================================
+// Translation of function get
+// ==================================================
+
+// Uninterpreted function definitions
+function  get(Heap: HeapType, r_1: Ref): Ref;
+function  get'(Heap: HeapType, r_1: Ref): Ref;
+axiom (forall Heap: HeapType, r_1: Ref ::
+  { get(Heap, r_1) }
+  get(Heap, r_1) == get'(Heap, r_1) && dummyFunction(get#triggerStateless(r_1))
+);
+axiom (forall Heap: HeapType, r_1: Ref ::
+  { get'(Heap, r_1) }
+  dummyFunction(get#triggerStateless(r_1))
+);
+
+// Framing axioms
+function  get#frame(frame: FrameType, r_1: Ref): Ref;
+axiom (forall Heap: HeapType, Mask: MaskType, r_1: Ref ::
+  { state(Heap, Mask), get'(Heap, r_1) }
+  state(Heap, Mask) ==> get'(Heap, r_1) == get#frame(EmptyFrame, r_1)
+);
+
+// Postcondition axioms
+axiom (forall Heap: HeapType, Mask: MaskType, r_1: Ref ::
+  { state(Heap, Mask), get'(Heap, r_1) }
+  state(Heap, Mask) && (AssumeFunctionsAbove < 3 || get#trigger(EmptyFrame, r_1)) ==> refs(Heap, r_1)[get'(Heap, r_1)]
+);
+
+// Trigger function (controlling recursive postconditions)
+function  get#trigger(frame: FrameType, r_1: Ref): bool;
+
+// State-independent trigger function
+function  get#triggerStateless(r_1: Ref): Ref;
+
+// Check contract well-formedness and postcondition
+procedure get#definedness(r_1: Ref) returns (Result: Ref)
+  modifies Heap, Mask;
+{
+  
+  // -- Initializing the state
+    Mask := ZeroMask;
+    assume state(Heap, Mask);
+    assume Heap[r_1, $allocated];
+    assume AssumeFunctionsAbove == 3;
+  
+  // -- Initializing the old state
+    assume Heap == old(Heap);
+    assume Mask == old(Mask);
+  
+  // -- Checking definedness of postcondition (no body)
+    
+    // -- Check definedness of (result in refs(r))
+      if (*) {
+        // Stop execution
+        assume false;
+      }
+      assume state(Heap, Mask);
+    assume state(Heap, Mask);
+    assume refs(Heap, r_1)[Result];
+    assume state(Heap, Mask);
+}
+
+// ==================================================
+// Translation of function tester
+// ==================================================
+
+// Uninterpreted function definitions
+function  tester(Heap: HeapType, r_1: Ref): Ref;
+function  tester'(Heap: HeapType, r_1: Ref): Ref;
+axiom (forall Heap: HeapType, r_1: Ref ::
+  { tester(Heap, r_1) }
+  tester(Heap, r_1) == tester'(Heap, r_1) && dummyFunction(tester#triggerStateless(r_1))
+);
+axiom (forall Heap: HeapType, r_1: Ref ::
+  { tester'(Heap, r_1) }
+  dummyFunction(tester#triggerStateless(r_1))
+);
+
+// Framing axioms
+function  tester#frame(frame: FrameType, r_1: Ref): Ref;
+axiom (forall Heap: HeapType, Mask: MaskType, r_1: Ref ::
+  { state(Heap, Mask), tester'(Heap, r_1) }
+  state(Heap, Mask) ==> tester'(Heap, r_1) == tester#frame(Heap[null, Q(r_1)], r_1)
+);
+
+// Trigger function (controlling recursive postconditions)
+function  tester#trigger(frame: FrameType, r_1: Ref): bool;
+
+// State-independent trigger function
+function  tester#triggerStateless(r_1: Ref): Ref;
+
+// Check contract well-formedness and postcondition
+procedure tester#definedness(r_1: Ref) returns (Result: Ref)
+  modifies Heap, Mask;
+{
+  var wildcard: real where wildcard > NoPerm;
+  var perm: Perm;
+  
+  // -- Initializing the state
+    Mask := ZeroMask;
+    assume state(Heap, Mask);
+    assume Heap[r_1, $allocated];
+    assume AssumeFunctionsAbove == 1;
+  
+  // -- Initializing the old state
+    assume Heap == old(Heap);
+    assume Mask == old(Mask);
+  
+  // -- Inhaling precondition (with checking)
+    havoc wildcard;
+    perm := wildcard;
+    Mask[null, Q(r_1)] := Mask[null, Q(r_1)] + perm;
+    assume state(Heap, Mask);
+    assume state(Heap, Mask);
+}
+
+// ==================================================
+// Translation of function testerFull
+// ==================================================
+
+// Uninterpreted function definitions
+function  testerFull(Heap: HeapType, r_1: Ref): Ref;
+function  testerFull'(Heap: HeapType, r_1: Ref): Ref;
+axiom (forall Heap: HeapType, r_1: Ref ::
+  { testerFull(Heap, r_1) }
+  testerFull(Heap, r_1) == testerFull'(Heap, r_1) && dummyFunction(testerFull#triggerStateless(r_1))
+);
+axiom (forall Heap: HeapType, r_1: Ref ::
+  { testerFull'(Heap, r_1) }
+  dummyFunction(testerFull#triggerStateless(r_1))
+);
+
+// Framing axioms
+function  testerFull#frame(frame: FrameType, r_1: Ref): Ref;
+axiom (forall Heap: HeapType, Mask: MaskType, r_1: Ref ::
+  { state(Heap, Mask), testerFull'(Heap, r_1) }
+  state(Heap, Mask) ==> testerFull'(Heap, r_1) == testerFull#frame(Heap[null, Q(r_1)], r_1)
+);
+
+// Trigger function (controlling recursive postconditions)
+function  testerFull#trigger(frame: FrameType, r_1: Ref): bool;
+
+// State-independent trigger function
+function  testerFull#triggerStateless(r_1: Ref): Ref;
+
+// Check contract well-formedness and postcondition
+procedure testerFull#definedness(r_1: Ref) returns (Result: Ref)
+  modifies Heap, Mask;
+{
+  var perm: Perm;
+  
+  // -- Initializing the state
+    Mask := ZeroMask;
+    assume state(Heap, Mask);
+    assume Heap[r_1, $allocated];
+    assume AssumeFunctionsAbove == 4;
+  
+  // -- Initializing the old state
+    assume Heap == old(Heap);
+    assume Mask == old(Mask);
+  
+  // -- Inhaling precondition (with checking)
+    perm := FullPerm;
+    Mask[null, Q(r_1)] := Mask[null, Q(r_1)] + perm;
+    assume state(Heap, Mask);
+    assume state(Heap, Mask);
+}
+
+// ==================================================
+// Translation of function testerfield
+// ==================================================
+
+// Uninterpreted function definitions
+function  testerfield(Heap: HeapType, r_1: Ref): Ref;
+function  testerfield'(Heap: HeapType, r_1: Ref): Ref;
+axiom (forall Heap: HeapType, r_1: Ref ::
+  { testerfield(Heap, r_1) }
+  testerfield(Heap, r_1) == testerfield'(Heap, r_1) && dummyFunction(testerfield#triggerStateless(r_1))
+);
+axiom (forall Heap: HeapType, r_1: Ref ::
+  { testerfield'(Heap, r_1) }
+  dummyFunction(testerfield#triggerStateless(r_1))
+);
+
+// Framing axioms
+function  testerfield#frame(frame: FrameType, r_1: Ref): Ref;
+axiom (forall Heap: HeapType, Mask: MaskType, r_1: Ref ::
+  { state(Heap, Mask), testerfield'(Heap, r_1) }
+  state(Heap, Mask) ==> testerfield'(Heap, r_1) == testerfield#frame(FrameFragment(Heap[r_1, q_1]), r_1)
+);
+
+// Trigger function (controlling recursive postconditions)
+function  testerfield#trigger(frame: FrameType, r_1: Ref): bool;
+
+// State-independent trigger function
+function  testerfield#triggerStateless(r_1: Ref): Ref;
+
+// Check contract well-formedness and postcondition
+procedure testerfield#definedness(r_1: Ref) returns (Result: Ref)
+  modifies Heap, Mask;
+{
+  var wildcard: real where wildcard > NoPerm;
+  var perm: Perm;
+  
+  // -- Initializing the state
+    Mask := ZeroMask;
+    assume state(Heap, Mask);
+    assume Heap[r_1, $allocated];
+    assume AssumeFunctionsAbove == 0;
+  
+  // -- Initializing the old state
+    assume Heap == old(Heap);
+    assume Mask == old(Mask);
+  
+  // -- Inhaling precondition (with checking)
+    havoc wildcard;
+    perm := wildcard;
+    assume r_1 != null;
+    Mask[r_1, q_1] := Mask[r_1, q_1] + perm;
+    assume state(Heap, Mask);
+    assume state(Heap, Mask);
+}
+
+// ==================================================
+// Translation of function testerfieldFull
+// ==================================================
+
+// Uninterpreted function definitions
+function  testerfieldFull(Heap: HeapType, r_1: Ref): Ref;
+function  testerfieldFull'(Heap: HeapType, r_1: Ref): Ref;
+axiom (forall Heap: HeapType, r_1: Ref ::
+  { testerfieldFull(Heap, r_1) }
+  testerfieldFull(Heap, r_1) == testerfieldFull'(Heap, r_1) && dummyFunction(testerfieldFull#triggerStateless(r_1))
+);
+axiom (forall Heap: HeapType, r_1: Ref ::
+  { testerfieldFull'(Heap, r_1) }
+  dummyFunction(testerfieldFull#triggerStateless(r_1))
+);
+
+// Framing axioms
+function  testerfieldFull#frame(frame: FrameType, r_1: Ref): Ref;
+axiom (forall Heap: HeapType, Mask: MaskType, r_1: Ref ::
+  { state(Heap, Mask), testerfieldFull'(Heap, r_1) }
+  state(Heap, Mask) ==> testerfieldFull'(Heap, r_1) == testerfieldFull#frame(FrameFragment(Heap[r_1, q_1]), r_1)
+);
+
+// Trigger function (controlling recursive postconditions)
+function  testerfieldFull#trigger(frame: FrameType, r_1: Ref): bool;
+
+// State-independent trigger function
+function  testerfieldFull#triggerStateless(r_1: Ref): Ref;
+
+// Check contract well-formedness and postcondition
+procedure testerfieldFull#definedness(r_1: Ref) returns (Result: Ref)
+  modifies Heap, Mask;
+{
+  var perm: Perm;
+  
+  // -- Initializing the state
+    Mask := ZeroMask;
+    assume state(Heap, Mask);
+    assume Heap[r_1, $allocated];
+    assume AssumeFunctionsAbove == 2;
+  
+  // -- Initializing the old state
+    assume Heap == old(Heap);
+    assume Mask == old(Mask);
+  
+  // -- Inhaling precondition (with checking)
+    perm := FullPerm;
+    assume r_1 != null;
+    Mask[r_1, q_1] := Mask[r_1, q_1] + perm;
+    assume state(Heap, Mask);
+    assume state(Heap, Mask);
+}
+
+// ==================================================
+// Translation of predicate P
+// ==================================================
+
+type PredicateType_P;
+function  P(r_1: Ref): Field PredicateType_P FrameType;
+function  P#sm(r_1: Ref): Field PredicateType_P PMaskType;
+axiom (forall r_1: Ref ::
+  { PredicateMaskField(P(r_1)) }
+  PredicateMaskField(P(r_1)) == P#sm(r_1)
+);
+axiom (forall r_1: Ref ::
+  { P(r_1) }
+  IsPredicateField(P(r_1))
+);
+axiom (forall r_1: Ref ::
+  { P(r_1) }
+  getPredicateId(P(r_1)) == 0
+);
+function  P#trigger<A>(Heap: HeapType, pred: (Field A FrameType)): bool;
+function  P#everUsed<A>(pred: (Field A FrameType)): bool;
+axiom (forall r_1: Ref, r2: Ref ::
+  { P(r_1), P(r2) }
+  P(r_1) == P(r2) ==> r_1 == r2
+);
+axiom (forall r_1: Ref, r2: Ref ::
+  { P#sm(r_1), P#sm(r2) }
+  P#sm(r_1) == P#sm(r2) ==> r_1 == r2
+);
+
+axiom (forall Heap: HeapType, r_1: Ref ::
+  { P#trigger(Heap, P(r_1)) }
+  P#everUsed(P(r_1))
+);
+
+// ==================================================
+// Function used for framing of quantified permission (forall e: Ref :: { (e in refs(r)) } (e in refs(r)) ==> acc(Q(e), wildcard)) in predicate P
+// ==================================================
+
+function  P#condqp1(Heap: HeapType, r_1_1: Ref): int;
+axiom (forall Heap2Heap: HeapType, Heap1Heap: HeapType, r_1: Ref ::
+  { P#condqp1(Heap2Heap, r_1), P#condqp1(Heap1Heap, r_1), succHeapTrans(Heap2Heap, Heap1Heap) }
+  (forall e: Ref ::
+    
+    (refs(Heap2Heap, r_1)[e] <==> refs(Heap1Heap, r_1)[e]) && (refs(Heap2Heap, r_1)[e] ==> Heap2Heap[null, Q(e)] == Heap1Heap[null, Q(e)])
+  ) ==> P#condqp1(Heap2Heap, r_1) == P#condqp1(Heap1Heap, r_1)
+);
+
+// ==================================================
+// Translation of predicate P2
+// ==================================================
+
+type PredicateType_P2;
+function  P2(r_1: Ref): Field PredicateType_P2 FrameType;
+function  P2#sm(r_1: Ref): Field PredicateType_P2 PMaskType;
+axiom (forall r_1: Ref ::
+  { PredicateMaskField(P2(r_1)) }
+  PredicateMaskField(P2(r_1)) == P2#sm(r_1)
+);
+axiom (forall r_1: Ref ::
+  { P2(r_1) }
+  IsPredicateField(P2(r_1))
+);
+axiom (forall r_1: Ref ::
+  { P2(r_1) }
+  getPredicateId(P2(r_1)) == 1
+);
+function  P2#trigger<A>(Heap: HeapType, pred: (Field A FrameType)): bool;
+function  P2#everUsed<A>(pred: (Field A FrameType)): bool;
+axiom (forall r_1: Ref, r2: Ref ::
+  { P2(r_1), P2(r2) }
+  P2(r_1) == P2(r2) ==> r_1 == r2
+);
+axiom (forall r_1: Ref, r2: Ref ::
+  { P2#sm(r_1), P2#sm(r2) }
+  P2#sm(r_1) == P2#sm(r2) ==> r_1 == r2
+);
+
+axiom (forall Heap: HeapType, r_1: Ref ::
+  { P2#trigger(Heap, P2(r_1)) }
+  P2#everUsed(P2(r_1))
+);
+
+// ==================================================
+// Function used for framing of quantified permission (forall e: Ref :: { (e in refs(r)) } (e in refs(r)) ==> acc(Q(e), 1 / 2)) in predicate P2
+// ==================================================
+
+function  P2#condqp2(Heap: HeapType, r_1_1: Ref): int;
+axiom (forall Heap2Heap: HeapType, Heap1Heap: HeapType, r_1: Ref ::
+  { P2#condqp2(Heap2Heap, r_1), P2#condqp2(Heap1Heap, r_1), succHeapTrans(Heap2Heap, Heap1Heap) }
+  (forall e: Ref ::
+    
+    (refs(Heap2Heap, r_1)[e] && NoPerm < 1 / 2 <==> refs(Heap1Heap, r_1)[e] && NoPerm < 1 / 2) && (refs(Heap2Heap, r_1)[e] && NoPerm < 1 / 2 ==> Heap2Heap[null, Q(e)] == Heap1Heap[null, Q(e)])
+  ) ==> P2#condqp2(Heap2Heap, r_1) == P2#condqp2(Heap1Heap, r_1)
+);
+
+// ==================================================
+// Translation of predicate R
+// ==================================================
+
+type PredicateType_R;
+function  R(r_1: Ref): Field PredicateType_R FrameType;
+function  R#sm(r_1: Ref): Field PredicateType_R PMaskType;
+axiom (forall r_1: Ref ::
+  { PredicateMaskField(R(r_1)) }
+  PredicateMaskField(R(r_1)) == R#sm(r_1)
+);
+axiom (forall r_1: Ref ::
+  { R(r_1) }
+  IsPredicateField(R(r_1))
+);
+axiom (forall r_1: Ref ::
+  { R(r_1) }
+  getPredicateId(R(r_1)) == 2
+);
+function  R#trigger<A>(Heap: HeapType, pred: (Field A FrameType)): bool;
+function  R#everUsed<A>(pred: (Field A FrameType)): bool;
+axiom (forall r_1: Ref, r2: Ref ::
+  { R(r_1), R(r2) }
+  R(r_1) == R(r2) ==> r_1 == r2
+);
+axiom (forall r_1: Ref, r2: Ref ::
+  { R#sm(r_1), R#sm(r2) }
+  R#sm(r_1) == R#sm(r2) ==> r_1 == r2
+);
+
+axiom (forall Heap: HeapType, r_1: Ref ::
+  { R#trigger(Heap, R(r_1)) }
+  R#everUsed(R(r_1))
+);
+
+// ==================================================
+// Function used for framing of quantified permission (forall e: Ref :: { (e in refs(r)) } (e in refs(r)) ==> acc(e.q, wildcard)) in predicate R
+// ==================================================
+
+function  R#condqp3(Heap: HeapType, r_1_1: Ref): int;
+axiom (forall Heap2Heap: HeapType, Heap1Heap: HeapType, r_1: Ref ::
+  { R#condqp3(Heap2Heap, r_1), R#condqp3(Heap1Heap, r_1), succHeapTrans(Heap2Heap, Heap1Heap) }
+  (forall e: Ref ::
+    
+    (refs(Heap2Heap, r_1)[e] <==> refs(Heap1Heap, r_1)[e]) && (refs(Heap2Heap, r_1)[e] ==> Heap2Heap[e, q_1] == Heap1Heap[e, q_1])
+  ) ==> R#condqp3(Heap2Heap, r_1) == R#condqp3(Heap1Heap, r_1)
+);
+
+// ==================================================
+// Translation of predicate R2
+// ==================================================
+
+type PredicateType_R2;
+function  R2(r_1: Ref): Field PredicateType_R2 FrameType;
+function  R2#sm(r_1: Ref): Field PredicateType_R2 PMaskType;
+axiom (forall r_1: Ref ::
+  { PredicateMaskField(R2(r_1)) }
+  PredicateMaskField(R2(r_1)) == R2#sm(r_1)
+);
+axiom (forall r_1: Ref ::
+  { R2(r_1) }
+  IsPredicateField(R2(r_1))
+);
+axiom (forall r_1: Ref ::
+  { R2(r_1) }
+  getPredicateId(R2(r_1)) == 3
+);
+function  R2#trigger<A>(Heap: HeapType, pred: (Field A FrameType)): bool;
+function  R2#everUsed<A>(pred: (Field A FrameType)): bool;
+axiom (forall r_1: Ref, r2: Ref ::
+  { R2(r_1), R2(r2) }
+  R2(r_1) == R2(r2) ==> r_1 == r2
+);
+axiom (forall r_1: Ref, r2: Ref ::
+  { R2#sm(r_1), R2#sm(r2) }
+  R2#sm(r_1) == R2#sm(r2) ==> r_1 == r2
+);
+
+axiom (forall Heap: HeapType, r_1: Ref ::
+  { R2#trigger(Heap, R2(r_1)) }
+  R2#everUsed(R2(r_1))
+);
+
+// ==================================================
+// Function used for framing of quantified permission (forall e: Ref :: { (e in refs(r)) } (e in refs(r)) ==> acc(e.q, 1 / 2)) in predicate R2
+// ==================================================
+
+function  R2#condqp4(Heap: HeapType, r_1_1: Ref): int;
+axiom (forall Heap2Heap: HeapType, Heap1Heap: HeapType, r_1: Ref ::
+  { R2#condqp4(Heap2Heap, r_1), R2#condqp4(Heap1Heap, r_1), succHeapTrans(Heap2Heap, Heap1Heap) }
+  (forall e: Ref ::
+    
+    (refs(Heap2Heap, r_1)[e] && NoPerm < 1 / 2 <==> refs(Heap1Heap, r_1)[e] && NoPerm < 1 / 2) && (refs(Heap2Heap, r_1)[e] && NoPerm < 1 / 2 ==> Heap2Heap[e, q_1] == Heap1Heap[e, q_1])
+  ) ==> R2#condqp4(Heap2Heap, r_1) == R2#condqp4(Heap1Heap, r_1)
+);
+
+// ==================================================
+// Translation of predicate Q
+// ==================================================
+
+type PredicateType_Q;
+function  Q(r_1: Ref): Field PredicateType_Q FrameType;
+function  Q#sm(r_1: Ref): Field PredicateType_Q PMaskType;
+axiom (forall r_1: Ref ::
+  { PredicateMaskField(Q(r_1)) }
+  PredicateMaskField(Q(r_1)) == Q#sm(r_1)
+);
+axiom (forall r_1: Ref ::
+  { Q(r_1) }
+  IsPredicateField(Q(r_1))
+);
+axiom (forall r_1: Ref ::
+  { Q(r_1) }
+  getPredicateId(Q(r_1)) == 4
+);
+function  Q#trigger<A>(Heap: HeapType, pred: (Field A FrameType)): bool;
+function  Q#everUsed<A>(pred: (Field A FrameType)): bool;
+axiom (forall r_1: Ref, r2: Ref ::
+  { Q(r_1), Q(r2) }
+  Q(r_1) == Q(r2) ==> r_1 == r2
+);
+axiom (forall r_1: Ref, r2: Ref ::
+  { Q#sm(r_1), Q#sm(r2) }
+  Q#sm(r_1) == Q#sm(r2) ==> r_1 == r2
+);
+
+axiom (forall Heap: HeapType, r_1: Ref ::
+  { Q#trigger(Heap, Q(r_1)) }
+  Q#everUsed(Q(r_1))
+);
+
+// ==================================================
+// Translation of method pred1
+// ==================================================
+
+procedure pred1(r_1: Ref) returns ()
+  modifies Heap, Mask;
+{
+  var wildcard: real where wildcard > NoPerm;
+  var perm: Perm;
+  var r2: Ref;
+  var newVersion: FrameType;
   var QPMask: MaskType;
-  var QPBMask: BMaskType;
-  var sWildcard: real;
+  var freshVersion: FrameType;
   var ExhaleHeap: HeapType;
   
   // -- Initializing the state
     Mask := ZeroMask;
-    BMask := ZeroBMask;
-    assume state(Heap, Mask, BMask);
+    assume state(Heap, Mask);
+    assume AssumeFunctionsAbove == -1;
+  
+  // -- Assumptions about method arguments
+    assume Heap[r_1, $allocated];
+  
+  // -- Checked inhaling of precondition
+    havoc wildcard;
+    perm := wildcard;
+    Mask[null, P(r_1)] := Mask[null, P(r_1)] + perm;
+    assume state(Heap, Mask);
+    assume state(Heap, Mask);
   
   // -- Initializing of old state
     
     // -- Initializing the old state
       assume Heap == old(Heap);
       assume Mask == old(Mask);
-      assume BMask == old(BMask);
   
   // -- Assumptions about local variables
-    assume Heap[x, $allocated];
-    assume Heap[y, $allocated];
+    assume Heap[r2, $allocated];
   
-  // -- Translating statement: inhale (forall r: Ref :: { (r in s) } (r in s) ==> acc(r.f, sWildcard)) -- test.vpr@5.11--7.5
+  // -- Translating statement: unfold acc(P(r), wildcard) -- 0196.vpr@32.17--33.5
+    assume P#trigger(Heap, P(r_1));
+    assume Heap[null, P(r_1)] == FrameFragment(P#condqp1(Heap, r_1));
+    // Phase 1: pure assertions and fixed permissions
     
-    // -- Check definedness of (forall r: Ref :: { (r in s) } (r in s) ==> acc(r.f, sWildcard))
-      if (*) {
-        assume false;
+    // -- Update version of predicate
+      if (!HasDirectPerm(Mask, null, P(r_1))) {
+        havoc newVersion;
+        Heap[null, P(r_1)] := newVersion;
       }
-      assume state(Heap, Mask, BMask);
+    // Phase 3: all remaining permissions (containing read permissions, but in a negative context)
+    perm := NoPerm;
+    havoc wildcard;
+    perm := perm + wildcard;
+    assert {:msg "  Unfolding P(r) might fail. There might be insufficient permission to access P(r) (0196.vpr@32.17--33.5) [120]"}
+      Mask[null, P(r_1)] > NoPerm;
+    assume wildcard < Mask[null, P(r_1)];
+    Mask[null, P(r_1)] := Mask[null, P(r_1)] - perm;
+    assume state(Heap, Mask);
     havoc QPMask;
-    havoc QPBMask;
+    havoc wildcard;
     
     // -- Define Inverse Function
-      assume (forall r_1: Ref ::
-        { Heap[r_1, f_6] } { QPMask[r_1, f_6] } { s[r_1] }
-        s[r_1] ==> qpRange1(r_1) && invRecv1(r_1) == r_1
+      assume (forall e: Ref ::
+        { Heap[null, Q(e)] } { Mask[null, Q(e)] } { refs(Heap, r_1)[e] }
+        refs(Heap, r_1)[e] ==> invRecv1(e) == e && qpRange1(e)
       );
-      assume (forall o_2: Ref ::
-        { invRecv1(o_2) }
-        s[invRecv1(o_2)] && qpRange1(o_2) ==> invRecv1(o_2) == o_2
-      );
-    
-    // -- Assume set of fields is nonNull
-      assume (forall r_1: Ref ::
-        { Heap[r_1, f_6] } { QPMask[r_1, f_6] } { s[r_1] }
-        s[r_1] ==> r_1 != null
+      assume (forall r_1_1: Ref ::
+        { invRecv1(r_1_1) }
+        (refs(Heap, r_1)[invRecv1(r_1_1)]) && qpRange1(r_1_1) ==> invRecv1(r_1_1) == r_1_1
       );
     
-    // -- Define permissions
-      assume (forall o_2: Ref ::
-        { QPMask[o_2, f_6] } { QPBMask[o_2, f_6] }
-        (s[invRecv1(o_2)] && qpRange1(o_2) ==> invRecv1(o_2) == o_2 && (QPMask[o_2, f_6] == Mask[o_2, f_6] && QPBMask[o_2, f_6])) && (!(s[invRecv1(o_2)] && qpRange1(o_2)) ==> QPMask[o_2, f_6] == Mask[o_2, f_6] && QPBMask[o_2, f_6] == BMask[o_2, f_6])
+    // -- Define updated permissions
+      assume (forall r_1_1: Ref ::
+        { QPMask[null, Q(r_1_1)] }
+        (refs(Heap, r_1)[invRecv1(r_1_1)]) && qpRange1(r_1_1) ==> (invRecv1(r_1_1) == r_1_1) && QPMask[null, Q(r_1_1)] == Mask[null, Q(r_1_1)] + wildcard
       );
+    
+    // -- Define independent locations
       assume (forall <A, B> o_2: Ref, f_4: (Field A B) ::
         { Mask[o_2, f_4] } { QPMask[o_2, f_4] }
-        f_4 != f_6 ==> Mask[o_2, f_4] == QPMask[o_2, f_4] && BMask[o_2, f_4] == QPBMask[o_2, f_4]
+        (o_2 != null || !IsPredicateField(f_4)) || getPredicateId(f_4) != 4 ==> Mask[o_2, f_4] == QPMask[o_2, f_4]
+      );
+      assume (forall r_1_1: Ref ::
+        { QPMask[null, Q(r_1_1)] }
+        !((refs(Heap, r_1)[invRecv1(r_1_1)]) && qpRange1(r_1_1)) ==> QPMask[null, Q(r_1_1)] == Mask[null, Q(r_1_1)]
       );
     Mask := QPMask;
-    BMask := QPBMask;
-    assume state(Heap, Mask, BMask);
-    assume state(Heap, Mask, BMask);
-    assume state(Heap, Mask, BMask);
+    assume state(Heap, Mask);
+    assume state(Heap, Mask);
+    assume state(Heap, Mask);
   
-  // -- Translating statement: inhale (x in s) -- test.vpr@10.13--11.5
-    assume s[x];
-    assume state(Heap, Mask, BMask);
-    assume state(Heap, Mask, BMask);
-  
-  // -- Translating statement: inhale (y in s) -- test.vpr@11.13--12.5
-    assume s[y];
-    assume state(Heap, Mask, BMask);
-    assume state(Heap, Mask, BMask);
-  
-  // -- Translating statement: inhale x != y -- test.vpr@12.13--14.5
-    assume x != y;
-    assume state(Heap, Mask, BMask);
-    assume state(Heap, Mask, BMask);
-  
-  // -- Translating statement: exhale (forall r: Ref :: { (r in s) } (r in s) ==> acc(r.f, sWildcard)) -- test.vpr@14.11--14.12
-    
-    // -- Check definedness of (forall r: Ref :: { (r in s) } (r in s) ==> acc(r.f, sWildcard))
-      if (*) {
-        assume false;
-      }
-      assume state(Heap, Mask, BMask);
+  // -- Translating statement: fold acc(P(r), wildcard) -- 0196.vpr@33.15--34.5
     // Phase 1: pure assertions and fixed permissions
     havoc QPMask;
-    havoc QPBMask;
-    // wild card assumptions
-    assert {:msg "  Exhale might fail. There might be insufficient permission to access r.f (test.vpr@14.11--14.12) [7]"}
-      (forall r_3: Ref ::
+    // wildcard assumptions
+    havoc wildcard;
+    assert {:msg "  Folding P(r) might fail. There might be insufficient permission to access Q(e) (0196.vpr@33.15--34.5) [121]"}
+      (forall e_2: Ref ::
       
-      s[r_3] ==> Mask[r_3, f_6] > NoPerm || BMask[r_3, f_6]
+      refs(Heap, r_1)[e_2] ==> Mask[null, Q(e_2)] > NoPerm
     );
+    assume (forall e_2: Ref ::
+      
+      refs(Heap, r_1)[e_2] ==> wildcard < Mask[null, Q(e_2)]
+    );
+  
     
-    // -- check if receiver r is injective
-      assert {:msg "  Exhale might fail. Receiver of r.f [test.vpr@14.57--14.57]  might not be injective. (test.vpr@14.11--14.12) [8]"}
-        (forall r_3: Ref, r_3_1: Ref ::
-        { neverTriggered2(r_3), neverTriggered2(r_3_1) }
-        (((r_3 != r_3_1 && s[r_3]) && s[r_3_1]) && NoPerm < sWildcard) && NoPerm < sWildcard ==> r_3 != r_3_1
+    // -- check if receiver acc(Q(e), wildcard * wildcard) is injective
+      assert {:msg "  Folding P(r) might fail. Receiver of Q(e) [0196.vpr@4.62--4.62]  might not be injective. (0196.vpr@33.15--34.5) [123]"}
+        (forall e_2: Ref, e_2_1: Ref ::
+        { neverTriggered2(e_2), neverTriggered2(e_2_1) }
+        (((e_2 != e_2_1 && refs(Heap, r_1)[e_2]) && refs(Heap, r_1)[e_2_1])) ==> e_2 != e_2_1
       );
     
     // -- check if sufficient permission is held
-      assert {:msg "  Exhale might fail. There might be insufficient permission to access r.f (test.vpr@14.11--14.12) [9]"}
-        (forall r_3: Ref ::
-        { Heap[r_3, f_6] } { QPMask[r_3, f_6] } { s[r_3] }
-        s[r_3] ==> Mask[r_3, f_6] > NoPerm || BMask[r_3, f_6]
+      assert {:msg "  Folding P(r) might fail. There might be insufficient permission to access Q(e) (0196.vpr@33.15--34.5) [124]"}
+        (forall e_2: Ref ::
+        { Heap[null, Q(e_2)] } { Mask[null, Q(e_2)] } { refs(Heap, r_1)[e_2] }
+        refs(Heap, r_1)[e_2] ==> Mask[null, Q(e_2)] > 0.000000000
       );
     
-    // -- assumptions for inverse of receiver r
-      assume (forall r_3: Ref ::
-        { Heap[r_3, f_6] } { QPMask[r_3, f_6] } { s[r_3] }
-        s[r_3] ==> qpRange2(r_3) && invRecv2(r_3) == r_3
+    // -- assumptions for inverse of receiver acc(Q(e), wildcard * wildcard)
+      assume (forall e_2: Ref ::
+        { Heap[null, Q(e_2)] } { Mask[null, Q(e_2)] } { refs(Heap, r_1)[e_2] }
+        refs(Heap, r_1)[e_2] ==> invRecv2(e_2) == e_2 && qpRange2(e_2)
       );
-      assume (forall o_2: Ref ::
-        { invRecv2(o_2) }
-        s[invRecv2(o_2)] && qpRange2(o_2) ==> invRecv2(o_2) == o_2
+      assume (forall r_2_1: Ref ::
+        { invRecv2(r_2_1) }
+        (refs(Heap, r_1)[invRecv2(r_2_1)] ) && qpRange2(r_2_1) ==> invRecv2(r_2_1) == r_2_1
       );
     
-    // -- assume permission updates for field f
+    // -- assume permission updates for predicate Q
+      assume (forall r_2_1: Ref ::
+        { QPMask[null, Q(r_2_1)] }
+        (refs(Heap, r_1)[invRecv2(r_2_1)] ) && qpRange2(r_2_1) ==> invRecv2(r_2_1) == r_2_1 && QPMask[null, Q(r_2_1)] == Mask[null, Q(r_2_1)] - wildcard
+      );
+      assume (forall r_2_1: Ref ::
+        { QPMask[null, Q(r_2_1)] }
+        !((refs(Heap, r_1)[invRecv2(r_2_1)] ) && qpRange2(r_2_1)) ==> QPMask[null, Q(r_2_1)] == Mask[null, Q(r_2_1)]
+      );
+    
+    // -- assume permission updates for independent locations 
+      assume (forall <A, B> o_2: Ref, f_4: (Field A B) ::
+        { Mask[o_2, f_4] } { QPMask[o_2, f_4] }
+        (o_2 != null || !IsPredicateField(f_4)) || getPredicateId(f_4) != 4 ==> Mask[o_2, f_4] == QPMask[o_2, f_4]
+      );
+    Mask := QPMask;
+    havoc wildcard;
+    perm := wildcard;
+    Mask[null, P(r_1)] := Mask[null, P(r_1)] + perm;
+    assume state(Heap, Mask);
+    assume state(Heap, Mask);
+    assume P#trigger(Heap, P(r_1));
+    assume Heap[null, P(r_1)] == FrameFragment(P#condqp1(Heap, r_1));
+    if (!HasDirectPerm(Mask, null, P(r_1))) {
+      Heap[null, P#sm(r_1)] := ZeroPMask;
+      havoc freshVersion;
+      Heap[null, P(r_1)] := freshVersion;
+    }
+    assume state(Heap, Mask);
+    assume state(Heap, Mask);
+  
+  // -- Translating statement: unfold acc(P(r), wildcard) -- 0196.vpr@34.17--35.5
+    assume P#trigger(Heap, P(r_1));
+    assume Heap[null, P(r_1)] == FrameFragment(P#condqp1(Heap, r_1));
+    // Phase 1: pure assertions and fixed permissions
+    
+    // -- Update version of predicate
+      if (!HasDirectPerm(Mask, null, P(r_1))) {
+        havoc newVersion;
+        Heap[null, P(r_1)] := newVersion;
+      }
+    // Phase 3: all remaining permissions (containing read permissions, but in a negative context)
+    perm := NoPerm;
+    havoc wildcard;
+    perm := perm + wildcard;
+    assert {:msg "  Unfolding P(r) might fail. There might be insufficient permission to access P(r) (0196.vpr@34.17--35.5) [125]"}
+      Mask[null, P(r_1)] > NoPerm;
+    assume wildcard < Mask[null, P(r_1)];
+    Mask[null, P(r_1)] := Mask[null, P(r_1)] - perm;
+    assume state(Heap, Mask);
+    havoc QPMask;
+    havoc wildcard;
+    
+    // -- Define Inverse Function
+      assume (forall e_3: Ref ::
+        { Heap[null, Q(e_3)] } { Mask[null, Q(e_3)] } { refs(Heap, r_1)[e_3] }
+        refs(Heap, r_1)[e_3] && NoPerm < wildcard ==> invRecv3(e_3) == e_3 && qpRange3(e_3)
+      );
+      assume (forall r_3_1: Ref ::
+        { invRecv3(r_3_1) }
+        (refs(Heap, r_1)[invRecv3(r_3_1)] && NoPerm < wildcard) && qpRange3(r_3_1) ==> invRecv3(r_3_1) == r_3_1
+      );
+    // Assume permission expression is non-negative for all fields
+    assume (forall e_3: Ref ::
+      { Heap[null, Q(e_3)] } { Mask[null, Q(e_3)] } { refs(Heap, r_1)[e_3] }
+      refs(Heap, r_1)[e_3] ==> wildcard >= NoPerm
+    );
+    
+    // -- Define updated permissions
+      assume (forall r_3_1: Ref ::
+        { QPMask[null, Q(r_3_1)] }
+        (refs(Heap, r_1)[invRecv3(r_3_1)] && NoPerm < wildcard) && qpRange3(r_3_1) ==> (NoPerm < wildcard ==> invRecv3(r_3_1) == r_3_1) && QPMask[null, Q(r_3_1)] == Mask[null, Q(r_3_1)] + wildcard
+      );
+    
+    // -- Define independent locations
+      assume (forall <A, B> o_2: Ref, f_4: (Field A B) ::
+        { Mask[o_2, f_4] } { QPMask[o_2, f_4] }
+        (o_2 != null || !IsPredicateField(f_4)) || getPredicateId(f_4) != 4 ==> Mask[o_2, f_4] == QPMask[o_2, f_4]
+      );
+      assume (forall r_3_1: Ref ::
+        { QPMask[null, Q(r_3_1)] }
+        !((refs(Heap, r_1)[invRecv3(r_3_1)] && NoPerm < wildcard) && qpRange3(r_3_1)) ==> QPMask[null, Q(r_3_1)] == Mask[null, Q(r_3_1)]
+      );
+    Mask := QPMask;
+    assume state(Heap, Mask);
+    assume state(Heap, Mask);
+    assume state(Heap, Mask);
+  
+  // -- Translating statement: r2 := tester(get(r)) -- 0196.vpr@35.8--38.1
+    
+    // -- Check definedness of tester(get(r))
+      if (*) {
+        // Stop execution
+        assume false;
+      }
+      if (*) {
+        // Exhale precondition of function application
+        // Phase 3: all remaining permissions (containing read permissions, but in a negative context)
+        perm := NoPerm;
+        havoc wildcard;
+        perm := perm + wildcard;
+        assert {:msg "  Precondition of function tester might not hold. There might be insufficient permission to access Q(get(r)) (0196.vpr@35.27--35.27) [126]"}
+          Mask[null, Q(get(Heap, r_1))] > NoPerm;
+        assume wildcard < Mask[null, Q(get(Heap, r_1))];
+        Mask[null, Q(get(Heap, r_1))] := Mask[null, Q(get(Heap, r_1))] - perm;
+        // Finish exhale
+        havoc ExhaleHeap;
+        assume IdenticalOnKnownLocations(Heap, ExhaleHeap, Mask);
+        Heap := ExhaleHeap;
+        // Stop execution
+        assume false;
+      }
+      assume state(Heap, Mask);
+    r2 := tester(Heap, get(Heap, r_1));
+    assume state(Heap, Mask);
+}
+
+// ==================================================
+// Translation of method pred2
+// ==================================================
+
+procedure pred2(r_1: Ref) returns ()
+  modifies Heap, Mask;
+{
+  var perm: Perm;
+  var r2: Ref;
+  var newVersion: FrameType;
+  var QPMask: MaskType;
+  var wildcard: real where wildcard > NoPerm;
+  var freshVersion: FrameType;
+  var ExhaleHeap: HeapType;
+  
+  // -- Initializing the state
+    Mask := ZeroMask;
+    assume state(Heap, Mask);
+    assume AssumeFunctionsAbove == -1;
+  
+  // -- Assumptions about method arguments
+    assume Heap[r_1, $allocated];
+  
+  // -- Checked inhaling of precondition
+    perm := FullPerm;
+    Mask[null, P(r_1)] := Mask[null, P(r_1)] + perm;
+    assume state(Heap, Mask);
+    assume state(Heap, Mask);
+  
+  // -- Initializing of old state
+    
+    // -- Initializing the old state
+      assume Heap == old(Heap);
+      assume Mask == old(Mask);
+  
+  // -- Assumptions about local variables
+    assume Heap[r2, $allocated];
+  
+  // -- Translating statement: unfold acc(P(r), write) -- 0196.vpr@43.17--44.5
+    assume P#trigger(Heap, P(r_1));
+    assume Heap[null, P(r_1)] == FrameFragment(P#condqp1(Heap, r_1));
+    // Phase 1: pure assertions and fixed permissions
+    perm := NoPerm;
+    perm := perm + FullPerm;
+    if (perm != NoPerm) {
+      assert {:msg "  Unfolding P(r) might fail. There might be insufficient permission to access P(r) (0196.vpr@43.17--44.5) [128]"}
+        perm <= Mask[null, P(r_1)];
+    }
+    Mask[null, P(r_1)] := Mask[null, P(r_1)] - perm;
+    
+    // -- Update version of predicate
+      if (!HasDirectPerm(Mask, null, P(r_1))) {
+        havoc newVersion;
+        Heap[null, P(r_1)] := newVersion;
+      }
+    assume state(Heap, Mask);
+    havoc QPMask;
+    havoc wildcard;
+    
+    // -- Define Inverse Function
+      assume (forall e: Ref ::
+        { Heap[null, Q(e)] } { Mask[null, Q(e)] } { refs(Heap, r_1)[e] }
+        refs(Heap, r_1)[e] && NoPerm < wildcard ==> invRecv4(e) == e && qpRange4(e)
+      );
+      assume (forall r_1_1: Ref ::
+        { invRecv4(r_1_1) }
+        (refs(Heap, r_1)[invRecv4(r_1_1)] && NoPerm < wildcard) && qpRange4(r_1_1) ==> invRecv4(r_1_1) == r_1_1
+      );
+    // Assume permission expression is non-negative for all fields
+    assume (forall e: Ref ::
+      { Heap[null, Q(e)] } { Mask[null, Q(e)] } { refs(Heap, r_1)[e] }
+      refs(Heap, r_1)[e] ==> wildcard >= NoPerm
+    );
+    
+    // -- Define updated permissions
+      assume (forall r_1_1: Ref ::
+        { QPMask[null, Q(r_1_1)] }
+        (refs(Heap, r_1)[invRecv4(r_1_1)] && NoPerm < wildcard) && qpRange4(r_1_1) ==> (NoPerm < wildcard ==> invRecv4(r_1_1) == r_1_1) && QPMask[null, Q(r_1_1)] == Mask[null, Q(r_1_1)] + wildcard
+      );
+    
+    // -- Define independent locations
+      assume (forall <A, B> o_2: Ref, f_4: (Field A B) ::
+        { Mask[o_2, f_4] } { QPMask[o_2, f_4] }
+        (o_2 != null || !IsPredicateField(f_4)) || getPredicateId(f_4) != 4 ==> Mask[o_2, f_4] == QPMask[o_2, f_4]
+      );
+      assume (forall r_1_1: Ref ::
+        { QPMask[null, Q(r_1_1)] }
+        !((refs(Heap, r_1)[invRecv4(r_1_1)] && NoPerm < wildcard) && qpRange4(r_1_1)) ==> QPMask[null, Q(r_1_1)] == Mask[null, Q(r_1_1)]
+      );
+    Mask := QPMask;
+    assume state(Heap, Mask);
+    assume state(Heap, Mask);
+    assume state(Heap, Mask);
+  
+  // -- Translating statement: fold acc(P(r), write) -- 0196.vpr@44.15--45.5
+    // Phase 1: pure assertions and fixed permissions
+    havoc QPMask;
+    // wildcard assumptions
+    havoc wildcard;
+    assert {:msg "  Folding P(r) might fail. There might be insufficient permission to access Q(e) (0196.vpr@44.15--45.5) [129]"}
+      (forall e_2: Ref ::
+      
+      refs(Heap, r_1)[e_2] ==> Mask[null, Q(e_2)] > NoPerm
+    );
+    assume (forall e_2: Ref ::
+      
+      refs(Heap, r_1)[e_2] ==> wildcard < Mask[null, Q(e_2)]
+    );
+    
+    // -- check that the permission amount is positive
+      assert {:msg "  Folding P(r) might fail. Fraction wildcard might be negative. (0196.vpr@44.15--45.5) [130]"}
+        (forall r_2_1: Ref ::
+        { invRecv5(r_2_1) }
+        refs(Heap, r_1)[invRecv5(r_2_1)] && qpRange5(r_2_1) ==> wildcard >= NoPerm
+      );
+    
+    // -- check if receiver acc(Q(e), wildcard) is injective
+      assert {:msg "  Folding P(r) might fail. Receiver of Q(e) [0196.vpr@4.62--4.62]  might not be injective. (0196.vpr@44.15--45.5) [131]"}
+        (forall e_2: Ref, e_2_1: Ref ::
+        { neverTriggered5(e_2), neverTriggered5(e_2_1) }
+        (((e_2 != e_2_1 && refs(Heap, r_1)[e_2]) && refs(Heap, r_1)[e_2_1]) && NoPerm < wildcard) && NoPerm < wildcard ==> e_2 != e_2_1
+      );
+    
+    // -- check if sufficient permission is held
+      assert {:msg "  Folding P(r) might fail. There might be insufficient permission to access Q(e) (0196.vpr@44.15--45.5) [132]"}
+        (forall e_2: Ref ::
+        { Heap[null, Q(e_2)] } { Mask[null, Q(e_2)] } { refs(Heap, r_1)[e_2] }
+        refs(Heap, r_1)[e_2] ==> Mask[null, Q(e_2)] > 0.000000000
+      );
+    
+    // -- assumptions for inverse of receiver acc(Q(e), wildcard)
+      assume (forall e_2: Ref ::
+        { Heap[null, Q(e_2)] } { Mask[null, Q(e_2)] } { refs(Heap, r_1)[e_2] }
+        refs(Heap, r_1)[e_2] && NoPerm < wildcard ==> invRecv5(e_2) == e_2 && qpRange5(e_2)
+      );
+      assume (forall r_2_1: Ref ::
+        { invRecv5(r_2_1) }
+        (refs(Heap, r_1)[invRecv5(r_2_1)] && NoPerm < wildcard) && qpRange5(r_2_1) ==> invRecv5(r_2_1) == r_2_1
+      );
+    
+    // -- assume permission updates for predicate Q
+      assume (forall r_2_1: Ref ::
+        { QPMask[null, Q(r_2_1)] }
+        (refs(Heap, r_1)[invRecv5(r_2_1)] && NoPerm < wildcard) && qpRange5(r_2_1) ==> invRecv5(r_2_1) == r_2_1 && QPMask[null, Q(r_2_1)] == Mask[null, Q(r_2_1)] - wildcard
+      );
+      assume (forall r_2_1: Ref ::
+        { QPMask[null, Q(r_2_1)] }
+        !((refs(Heap, r_1)[invRecv5(r_2_1)] && NoPerm < wildcard) && qpRange5(r_2_1)) ==> QPMask[null, Q(r_2_1)] == Mask[null, Q(r_2_1)]
+      );
+    
+    // -- assume permission updates for independent locations 
+      assume (forall <A, B> o_2: Ref, f_4: (Field A B) ::
+        { Mask[o_2, f_4] } { QPMask[o_2, f_4] }
+        (o_2 != null || !IsPredicateField(f_4)) || getPredicateId(f_4) != 4 ==> Mask[o_2, f_4] == QPMask[o_2, f_4]
+      );
+    Mask := QPMask;
+    perm := FullPerm;
+    Mask[null, P(r_1)] := Mask[null, P(r_1)] + perm;
+    assume state(Heap, Mask);
+    assume state(Heap, Mask);
+    assume P#trigger(Heap, P(r_1));
+    assume Heap[null, P(r_1)] == FrameFragment(P#condqp1(Heap, r_1));
+    if (!HasDirectPerm(Mask, null, P(r_1))) {
+      Heap[null, P#sm(r_1)] := ZeroPMask;
+      havoc freshVersion;
+      Heap[null, P(r_1)] := freshVersion;
+    }
+    assume state(Heap, Mask);
+    assume state(Heap, Mask);
+  
+  // -- Translating statement: unfold acc(P(r), write) -- 0196.vpr@45.17--46.5
+    assume P#trigger(Heap, P(r_1));
+    assume Heap[null, P(r_1)] == FrameFragment(P#condqp1(Heap, r_1));
+    // Phase 1: pure assertions and fixed permissions
+    perm := NoPerm;
+    perm := perm + FullPerm;
+    if (perm != NoPerm) {
+      assert {:msg "  Unfolding P(r) might fail. There might be insufficient permission to access P(r) (0196.vpr@45.17--46.5) [134]"}
+        perm <= Mask[null, P(r_1)];
+    }
+    Mask[null, P(r_1)] := Mask[null, P(r_1)] - perm;
+    
+    // -- Update version of predicate
+      if (!HasDirectPerm(Mask, null, P(r_1))) {
+        havoc newVersion;
+        Heap[null, P(r_1)] := newVersion;
+      }
+    assume state(Heap, Mask);
+    havoc QPMask;
+    havoc wildcard;
+    
+    // -- Define Inverse Function
+      assume (forall e_3: Ref ::
+        { Heap[null, Q(e_3)] } { Mask[null, Q(e_3)] } { refs(Heap, r_1)[e_3] }
+        refs(Heap, r_1)[e_3] && NoPerm < wildcard ==> invRecv6(e_3) == e_3 && qpRange6(e_3)
+      );
+      assume (forall r_3_1: Ref ::
+        { invRecv6(r_3_1) }
+        (refs(Heap, r_1)[invRecv6(r_3_1)] && NoPerm < wildcard) && qpRange6(r_3_1) ==> invRecv6(r_3_1) == r_3_1
+      );
+    // Assume permission expression is non-negative for all fields
+    assume (forall e_3: Ref ::
+      { Heap[null, Q(e_3)] } { Mask[null, Q(e_3)] } { refs(Heap, r_1)[e_3] }
+      refs(Heap, r_1)[e_3] ==> wildcard >= NoPerm
+    );
+    
+    // -- Define updated permissions
+      assume (forall r_3_1: Ref ::
+        { QPMask[null, Q(r_3_1)] }
+        (refs(Heap, r_1)[invRecv6(r_3_1)] && NoPerm < wildcard) && qpRange6(r_3_1) ==> (NoPerm < wildcard ==> invRecv6(r_3_1) == r_3_1) && QPMask[null, Q(r_3_1)] == Mask[null, Q(r_3_1)] + wildcard
+      );
+    
+    // -- Define independent locations
+      assume (forall <A, B> o_2: Ref, f_4: (Field A B) ::
+        { Mask[o_2, f_4] } { QPMask[o_2, f_4] }
+        (o_2 != null || !IsPredicateField(f_4)) || getPredicateId(f_4) != 4 ==> Mask[o_2, f_4] == QPMask[o_2, f_4]
+      );
+      assume (forall r_3_1: Ref ::
+        { QPMask[null, Q(r_3_1)] }
+        !((refs(Heap, r_1)[invRecv6(r_3_1)] && NoPerm < wildcard) && qpRange6(r_3_1)) ==> QPMask[null, Q(r_3_1)] == Mask[null, Q(r_3_1)]
+      );
+    Mask := QPMask;
+    assume state(Heap, Mask);
+    assume state(Heap, Mask);
+    assume state(Heap, Mask);
+  
+  // -- Translating statement: r2 := tester(get(r)) -- 0196.vpr@46.8--49.1
+    
+    // -- Check definedness of tester(get(r))
+      if (*) {
+        // Stop execution
+        assume false;
+      }
+      if (*) {
+        // Exhale precondition of function application
+        // Phase 3: all remaining permissions (containing read permissions, but in a negative context)
+        perm := NoPerm;
+        havoc wildcard;
+        perm := perm + wildcard;
+        assert {:msg "  Precondition of function tester might not hold. There might be insufficient permission to access Q(get(r)) (0196.vpr@46.27--46.27) [135]"}
+          Mask[null, Q(get(Heap, r_1))] > NoPerm;
+        assume wildcard < Mask[null, Q(get(Heap, r_1))];
+        Mask[null, Q(get(Heap, r_1))] := Mask[null, Q(get(Heap, r_1))] - perm;
+        // Finish exhale
+        havoc ExhaleHeap;
+        assume IdenticalOnKnownLocations(Heap, ExhaleHeap, Mask);
+        Heap := ExhaleHeap;
+        // Stop execution
+        assume false;
+      }
+      assume state(Heap, Mask);
+    r2 := tester(Heap, get(Heap, r_1));
+    assume state(Heap, Mask);
+}
+
+// ==================================================
+// Translation of method pred3
+// ==================================================
+
+procedure pred3(r_1: Ref) returns ()
+  modifies Heap, Mask;
+{
+  var perm: Perm;
+  var r2: Ref;
+  var newVersion: FrameType;
+  var QPMask: MaskType;
+  var wildcard: real where wildcard > NoPerm;
+  var freshVersion: FrameType;
+  var ExhaleHeap: HeapType;
+  
+  // -- Initializing the state
+    Mask := ZeroMask;
+    assume state(Heap, Mask);
+    assume AssumeFunctionsAbove == -1;
+  
+  // -- Assumptions about method arguments
+    assume Heap[r_1, $allocated];
+  
+  // -- Checked inhaling of precondition
+    perm := FullPerm;
+    Mask[null, P(r_1)] := Mask[null, P(r_1)] + perm;
+    assume state(Heap, Mask);
+    assume state(Heap, Mask);
+  
+  // -- Initializing of old state
+    
+    // -- Initializing the old state
+      assume Heap == old(Heap);
+      assume Mask == old(Mask);
+  
+  // -- Assumptions about local variables
+    assume Heap[r2, $allocated];
+  
+  // -- Translating statement: unfold acc(P(r), 1 / 2) -- 0196.vpr@54.17--55.5
+    assume P#trigger(Heap, P(r_1));
+    assume Heap[null, P(r_1)] == FrameFragment(P#condqp1(Heap, r_1));
+    // Phase 1: pure assertions and fixed permissions
+    assert {:msg "  Unfolding P(r) might fail. Fraction 1 / 2 might be negative. (0196.vpr@54.17--55.5) [136]"}
+      1 / 2 >= NoPerm;
+    perm := NoPerm;
+    perm := perm + 1 / 2;
+    if (perm != NoPerm) {
+      assert {:msg "  Unfolding P(r) might fail. There might be insufficient permission to access P(r) (0196.vpr@54.17--55.5) [137]"}
+        perm <= Mask[null, P(r_1)];
+    }
+    Mask[null, P(r_1)] := Mask[null, P(r_1)] - perm;
+    
+    // -- Update version of predicate
+      if (!HasDirectPerm(Mask, null, P(r_1))) {
+        havoc newVersion;
+        Heap[null, P(r_1)] := newVersion;
+      }
+    assume state(Heap, Mask);
+    havoc QPMask;
+    havoc wildcard;
+    
+    // -- Define Inverse Function
+      assume (forall e: Ref ::
+        { Heap[null, Q(e)] } { Mask[null, Q(e)] } { refs(Heap, r_1)[e] }
+        refs(Heap, r_1)[e] && NoPerm < wildcard ==> invRecv7(e) == e && qpRange7(e)
+      );
+      assume (forall r_1_1: Ref ::
+        { invRecv7(r_1_1) }
+        (refs(Heap, r_1)[invRecv7(r_1_1)] && NoPerm < wildcard) && qpRange7(r_1_1) ==> invRecv7(r_1_1) == r_1_1
+      );
+    // Assume permission expression is non-negative for all fields
+    assume (forall e: Ref ::
+      { Heap[null, Q(e)] } { Mask[null, Q(e)] } { refs(Heap, r_1)[e] }
+      refs(Heap, r_1)[e] ==> wildcard >= NoPerm
+    );
+    
+    // -- Define updated permissions
+      assume (forall r_1_1: Ref ::
+        { QPMask[null, Q(r_1_1)] }
+        (refs(Heap, r_1)[invRecv7(r_1_1)] && NoPerm < wildcard) && qpRange7(r_1_1) ==> (NoPerm < wildcard ==> invRecv7(r_1_1) == r_1_1) && QPMask[null, Q(r_1_1)] == Mask[null, Q(r_1_1)] + wildcard
+      );
+    
+    // -- Define independent locations
+      assume (forall <A, B> o_2: Ref, f_4: (Field A B) ::
+        { Mask[o_2, f_4] } { QPMask[o_2, f_4] }
+        (o_2 != null || !IsPredicateField(f_4)) || getPredicateId(f_4) != 4 ==> Mask[o_2, f_4] == QPMask[o_2, f_4]
+      );
+      assume (forall r_1_1: Ref ::
+        { QPMask[null, Q(r_1_1)] }
+        !((refs(Heap, r_1)[invRecv7(r_1_1)] && NoPerm < wildcard) && qpRange7(r_1_1)) ==> QPMask[null, Q(r_1_1)] == Mask[null, Q(r_1_1)]
+      );
+    Mask := QPMask;
+    assume state(Heap, Mask);
+    assume state(Heap, Mask);
+    assume state(Heap, Mask);
+  
+  // -- Translating statement: fold acc(P(r), 1 / 2) -- 0196.vpr@55.15--56.5
+    // Phase 1: pure assertions and fixed permissions
+    havoc QPMask;
+    // wildcard assumptions
+    havoc wildcard;
+    assert {:msg "  Folding P(r) might fail. There might be insufficient permission to access Q(e) (0196.vpr@55.15--56.5) [138]"}
+      (forall e_2: Ref ::
+      
+      refs(Heap, r_1)[e_2] ==> Mask[null, Q(e_2)] > NoPerm
+    );
+    assume (forall e_2: Ref ::
+      
+      refs(Heap, r_1)[e_2] ==> wildcard < Mask[null, Q(e_2)]
+    );
+    
+    // -- check that the permission amount is positive
+      assert {:msg "  Folding P(r) might fail. Fraction wildcard * (1 / 2) might be negative. (0196.vpr@55.15--56.5) [139]"}
+        (forall r_2_1: Ref ::
+        { invRecv8(r_2_1) }
+        refs(Heap, r_1)[invRecv8(r_2_1)] && qpRange8(r_2_1) ==> wildcard >= NoPerm
+      );
+    
+    // -- check if receiver acc(Q(e), wildcard * (1 / 2)) is injective
+      assert {:msg "  Folding P(r) might fail. Receiver of Q(e) [0196.vpr@4.62--4.62]  might not be injective. (0196.vpr@55.15--56.5) [140]"}
+        (forall e_2: Ref, e_2_1: Ref ::
+        { neverTriggered8(e_2), neverTriggered8(e_2_1) }
+        (((e_2 != e_2_1 && refs(Heap, r_1)[e_2]) && refs(Heap, r_1)[e_2_1]) && NoPerm < wildcard) && NoPerm < wildcard ==> e_2 != e_2_1
+      );
+    
+    // -- check if sufficient permission is held
+      assert {:msg "  Folding P(r) might fail. There might be insufficient permission to access Q(e) (0196.vpr@55.15--56.5) [141]"}
+        (forall e_2: Ref ::
+        { Heap[null, Q(e_2)] } { Mask[null, Q(e_2)] } { refs(Heap, r_1)[e_2] }
+        refs(Heap, r_1)[e_2] ==> Mask[null, Q(e_2)] > 0.000000000
+      );
+    
+    // -- assumptions for inverse of receiver acc(Q(e), wildcard * (1 / 2))
+      assume (forall e_2: Ref ::
+        { Heap[null, Q(e_2)] } { Mask[null, Q(e_2)] } { refs(Heap, r_1)[e_2] }
+        refs(Heap, r_1)[e_2] && NoPerm < wildcard ==> invRecv8(e_2) == e_2 && qpRange8(e_2)
+      );
+      assume (forall r_2_1: Ref ::
+        { invRecv8(r_2_1) }
+        (refs(Heap, r_1)[invRecv8(r_2_1)] && NoPerm < wildcard) && qpRange8(r_2_1) ==> invRecv8(r_2_1) == r_2_1
+      );
+    
+    // -- assume permission updates for predicate Q
+      assume (forall r_2_1: Ref ::
+        { QPMask[null, Q(r_2_1)] }
+        (refs(Heap, r_1)[invRecv8(r_2_1)] && NoPerm < wildcard) && qpRange8(r_2_1) ==> invRecv8(r_2_1) == r_2_1 && QPMask[null, Q(r_2_1)] == Mask[null, Q(r_2_1)] - wildcard
+      );
+      assume (forall r_2_1: Ref ::
+        { QPMask[null, Q(r_2_1)] }
+        !((refs(Heap, r_1)[invRecv8(r_2_1)] && NoPerm < wildcard) && qpRange8(r_2_1)) ==> QPMask[null, Q(r_2_1)] == Mask[null, Q(r_2_1)]
+      );
+    
+    // -- assume permission updates for independent locations 
+      assume (forall <A, B> o_2: Ref, f_4: (Field A B) ::
+        { Mask[o_2, f_4] } { QPMask[o_2, f_4] }
+        (o_2 != null || !IsPredicateField(f_4)) || getPredicateId(f_4) != 4 ==> Mask[o_2, f_4] == QPMask[o_2, f_4]
+      );
+    Mask := QPMask;
+    perm := 1 / 2;
+    assume perm >= NoPerm;
+    Mask[null, P(r_1)] := Mask[null, P(r_1)] + perm;
+    assume state(Heap, Mask);
+    assume state(Heap, Mask);
+    assume P#trigger(Heap, P(r_1));
+    assume Heap[null, P(r_1)] == FrameFragment(P#condqp1(Heap, r_1));
+    if (!HasDirectPerm(Mask, null, P(r_1))) {
+      Heap[null, P#sm(r_1)] := ZeroPMask;
+      havoc freshVersion;
+      Heap[null, P(r_1)] := freshVersion;
+    }
+    assume state(Heap, Mask);
+    assume state(Heap, Mask);
+  
+  // -- Translating statement: unfold acc(P(r), 1 / 2) -- 0196.vpr@56.17--57.5
+    assume P#trigger(Heap, P(r_1));
+    assume Heap[null, P(r_1)] == FrameFragment(P#condqp1(Heap, r_1));
+    // Phase 1: pure assertions and fixed permissions
+    assert {:msg "  Unfolding P(r) might fail. Fraction 1 / 2 might be negative. (0196.vpr@56.17--57.5) [142]"}
+      1 / 2 >= NoPerm;
+    perm := NoPerm;
+    perm := perm + 1 / 2;
+    if (perm != NoPerm) {
+      assert {:msg "  Unfolding P(r) might fail. There might be insufficient permission to access P(r) (0196.vpr@56.17--57.5) [143]"}
+        perm <= Mask[null, P(r_1)];
+    }
+    Mask[null, P(r_1)] := Mask[null, P(r_1)] - perm;
+    
+    // -- Update version of predicate
+      if (!HasDirectPerm(Mask, null, P(r_1))) {
+        havoc newVersion;
+        Heap[null, P(r_1)] := newVersion;
+      }
+    assume state(Heap, Mask);
+    havoc QPMask;
+    havoc wildcard;
+    
+    // -- Define Inverse Function
+      assume (forall e_3: Ref ::
+        { Heap[null, Q(e_3)] } { Mask[null, Q(e_3)] } { refs(Heap, r_1)[e_3] }
+        refs(Heap, r_1)[e_3] && NoPerm < wildcard ==> invRecv9(e_3) == e_3 && qpRange9(e_3)
+      );
+      assume (forall r_3_1: Ref ::
+        { invRecv9(r_3_1) }
+        (refs(Heap, r_1)[invRecv9(r_3_1)] && NoPerm < wildcard) && qpRange9(r_3_1) ==> invRecv9(r_3_1) == r_3_1
+      );
+    // Assume permission expression is non-negative for all fields
+    assume (forall e_3: Ref ::
+      { Heap[null, Q(e_3)] } { Mask[null, Q(e_3)] } { refs(Heap, r_1)[e_3] }
+      refs(Heap, r_1)[e_3] ==> wildcard >= NoPerm
+    );
+    
+    // -- Define updated permissions
+      assume (forall r_3_1: Ref ::
+        { QPMask[null, Q(r_3_1)] }
+        (refs(Heap, r_1)[invRecv9(r_3_1)] && NoPerm < wildcard) && qpRange9(r_3_1) ==> (NoPerm < wildcard ==> invRecv9(r_3_1) == r_3_1) && QPMask[null, Q(r_3_1)] == Mask[null, Q(r_3_1)] + wildcard
+      );
+    
+    // -- Define independent locations
+      assume (forall <A, B> o_2: Ref, f_4: (Field A B) ::
+        { Mask[o_2, f_4] } { QPMask[o_2, f_4] }
+        (o_2 != null || !IsPredicateField(f_4)) || getPredicateId(f_4) != 4 ==> Mask[o_2, f_4] == QPMask[o_2, f_4]
+      );
+      assume (forall r_3_1: Ref ::
+        { QPMask[null, Q(r_3_1)] }
+        !((refs(Heap, r_1)[invRecv9(r_3_1)] && NoPerm < wildcard) && qpRange9(r_3_1)) ==> QPMask[null, Q(r_3_1)] == Mask[null, Q(r_3_1)]
+      );
+    Mask := QPMask;
+    assume state(Heap, Mask);
+    assume state(Heap, Mask);
+    assume state(Heap, Mask);
+  
+  // -- Translating statement: r2 := tester(get(r)) -- 0196.vpr@57.8--60.1
+    
+    // -- Check definedness of tester(get(r))
+      if (*) {
+        // Stop execution
+        assume false;
+      }
+      if (*) {
+        // Exhale precondition of function application
+        // Phase 3: all remaining permissions (containing read permissions, but in a negative context)
+        perm := NoPerm;
+        havoc wildcard;
+        perm := perm + wildcard;
+        assert {:msg "  Precondition of function tester might not hold. There might be insufficient permission to access Q(get(r)) (0196.vpr@57.27--57.27) [144]"}
+          Mask[null, Q(get(Heap, r_1))] > NoPerm;
+        assume wildcard < Mask[null, Q(get(Heap, r_1))];
+        Mask[null, Q(get(Heap, r_1))] := Mask[null, Q(get(Heap, r_1))] - perm;
+        // Finish exhale
+        havoc ExhaleHeap;
+        assume IdenticalOnKnownLocations(Heap, ExhaleHeap, Mask);
+        Heap := ExhaleHeap;
+        // Stop execution
+        assume false;
+      }
+      assume state(Heap, Mask);
+    r2 := tester(Heap, get(Heap, r_1));
+    assume state(Heap, Mask);
+}
+
+// ==================================================
+// Translation of method pred4
+// ==================================================
+
+procedure pred4(r_1: Ref) returns ()
+  modifies Heap, Mask;
+{
+  var perm: Perm;
+  var r2: Ref;
+  var newVersion: FrameType;
+  var wildcard: real where wildcard > NoPerm;
+  var QPMask: MaskType;
+  var freshVersion: FrameType;
+  var ExhaleHeap: HeapType;
+  
+  // -- Initializing the state
+    Mask := ZeroMask;
+    assume state(Heap, Mask);
+    assume AssumeFunctionsAbove == -1;
+  
+  // -- Assumptions about method arguments
+    assume Heap[r_1, $allocated];
+  
+  // -- Checked inhaling of precondition
+    perm := FullPerm;
+    Mask[null, P2(r_1)] := Mask[null, P2(r_1)] + perm;
+    assume state(Heap, Mask);
+    assume state(Heap, Mask);
+  
+  // -- Initializing of old state
+    
+    // -- Initializing the old state
+      assume Heap == old(Heap);
+      assume Mask == old(Mask);
+  
+  // -- Assumptions about local variables
+    assume Heap[r2, $allocated];
+  
+  // -- Translating statement: unfold acc(P2(r), wildcard) -- 0196.vpr@65.18--66.5
+    assume P2#trigger(Heap, P2(r_1));
+    assume Heap[null, P2(r_1)] == FrameFragment(P2#condqp2(Heap, r_1));
+    // Phase 1: pure assertions and fixed permissions
+    
+    // -- Update version of predicate
+      if (!HasDirectPerm(Mask, null, P2(r_1))) {
+        havoc newVersion;
+        Heap[null, P2(r_1)] := newVersion;
+      }
+    // Phase 3: all remaining permissions (containing read permissions, but in a negative context)
+    perm := NoPerm;
+    havoc wildcard;
+    perm := perm + wildcard;
+    assert {:msg "  Unfolding P2(r) might fail. There might be insufficient permission to access P2(r) (0196.vpr@65.18--66.5) [145]"}
+      Mask[null, P2(r_1)] > NoPerm;
+    assume wildcard < Mask[null, P2(r_1)];
+    Mask[null, P2(r_1)] := Mask[null, P2(r_1)] - perm;
+    assume state(Heap, Mask);
+    havoc QPMask;
+    havoc wildcard;
+    
+    // -- Define Inverse Function
+      assume (forall e: Ref ::
+        { Heap[null, Q(e)] } { Mask[null, Q(e)] } { refs(Heap, r_1)[e] }
+        refs(Heap, r_1)[e] && NoPerm < wildcard ==> invRecv10(e) == e && qpRange10(e)
+      );
+      assume (forall r_1_1: Ref ::
+        { invRecv10(r_1_1) }
+        (refs(Heap, r_1)[invRecv10(r_1_1)] && NoPerm < wildcard) && qpRange10(r_1_1) ==> invRecv10(r_1_1) == r_1_1
+      );
+    // Assume permission expression is non-negative for all fields
+    assume (forall e: Ref ::
+      { Heap[null, Q(e)] } { Mask[null, Q(e)] } { refs(Heap, r_1)[e] }
+      refs(Heap, r_1)[e] ==> wildcard >= NoPerm
+    );
+    
+    // -- Define updated permissions
+      assume (forall r_1_1: Ref ::
+        { QPMask[null, Q(r_1_1)] }
+        (refs(Heap, r_1)[invRecv10(r_1_1)] && NoPerm < wildcard) && qpRange10(r_1_1) ==> (NoPerm < wildcard ==> invRecv10(r_1_1) == r_1_1) && QPMask[null, Q(r_1_1)] == Mask[null, Q(r_1_1)] + wildcard
+      );
+    
+    // -- Define independent locations
+      assume (forall <A, B> o_2: Ref, f_4: (Field A B) ::
+        { Mask[o_2, f_4] } { QPMask[o_2, f_4] }
+        (o_2 != null || !IsPredicateField(f_4)) || getPredicateId(f_4) != 4 ==> Mask[o_2, f_4] == QPMask[o_2, f_4]
+      );
+      assume (forall r_1_1: Ref ::
+        { QPMask[null, Q(r_1_1)] }
+        !((refs(Heap, r_1)[invRecv10(r_1_1)] && NoPerm < wildcard) && qpRange10(r_1_1)) ==> QPMask[null, Q(r_1_1)] == Mask[null, Q(r_1_1)]
+      );
+    Mask := QPMask;
+    assume state(Heap, Mask);
+    assume state(Heap, Mask);
+    assume state(Heap, Mask);
+  
+  // -- Translating statement: fold acc(P2(r), wildcard) -- 0196.vpr@66.16--67.5
+    // Phase 1: pure assertions and fixed permissions
+    havoc QPMask;
+    // wildcard assumptions
+    havoc wildcard;
+    assert {:msg "  Folding P2(r) might fail. There might be insufficient permission to access Q(e) (0196.vpr@66.16--67.5) [146]"}
+      (forall e_2: Ref ::
+      
+      refs(Heap, r_1)[e_2] ==> Mask[null, Q(e_2)] > NoPerm
+    );
+    assume (forall e_2: Ref ::
+      
+      refs(Heap, r_1)[e_2] ==> wildcard < Mask[null, Q(e_2)]
+    );
+    
+    // -- check that the permission amount is positive
+      assert {:msg "  Folding P2(r) might fail. Fraction 1 / 2 * wildcard might be negative. (0196.vpr@66.16--67.5) [147]"}
+        (forall r_2_1: Ref ::
+        { invRecv11(r_2_1) }
+        refs(Heap, r_1)[invRecv11(r_2_1)] && qpRange11(r_2_1) ==> wildcard >= NoPerm
+      );
+    
+    // -- check if receiver acc(Q(e), 1 / 2 * wildcard) is injective
+      assert {:msg "  Folding P2(r) might fail. Receiver of Q(e) [0196.vpr@5.63--5.63]  might not be injective. (0196.vpr@66.16--67.5) [148]"}
+        (forall e_2: Ref, e_2_1: Ref ::
+        { neverTriggered11(e_2), neverTriggered11(e_2_1) }
+        (((e_2 != e_2_1 && refs(Heap, r_1)[e_2]) && refs(Heap, r_1)[e_2_1]) && NoPerm < wildcard) && NoPerm < wildcard ==> e_2 != e_2_1
+      );
+    
+    // -- check if sufficient permission is held
+      assert {:msg "  Folding P2(r) might fail. There might be insufficient permission to access Q(e) (0196.vpr@66.16--67.5) [149]"}
+        (forall e_2: Ref ::
+        { Heap[null, Q(e_2)] } { Mask[null, Q(e_2)] } { refs(Heap, r_1)[e_2] }
+        refs(Heap, r_1)[e_2] ==> Mask[null, Q(e_2)] > 0.000000000
+      );
+    
+    // -- assumptions for inverse of receiver acc(Q(e), 1 / 2 * wildcard)
+      assume (forall e_2: Ref ::
+        { Heap[null, Q(e_2)] } { Mask[null, Q(e_2)] } { refs(Heap, r_1)[e_2] }
+        refs(Heap, r_1)[e_2] && NoPerm < wildcard ==> invRecv11(e_2) == e_2 && qpRange11(e_2)
+      );
+      assume (forall r_2_1: Ref ::
+        { invRecv11(r_2_1) }
+        (refs(Heap, r_1)[invRecv11(r_2_1)] && NoPerm < wildcard) && qpRange11(r_2_1) ==> invRecv11(r_2_1) == r_2_1
+      );
+    
+    // -- assume permission updates for predicate Q
+      assume (forall r_2_1: Ref ::
+        { QPMask[null, Q(r_2_1)] }
+        (refs(Heap, r_1)[invRecv11(r_2_1)] && NoPerm < wildcard) && qpRange11(r_2_1) ==> invRecv11(r_2_1) == r_2_1 && QPMask[null, Q(r_2_1)] == Mask[null, Q(r_2_1)] - wildcard
+      );
+      assume (forall r_2_1: Ref ::
+        { QPMask[null, Q(r_2_1)] }
+        !((refs(Heap, r_1)[invRecv11(r_2_1)] && NoPerm < wildcard) && qpRange11(r_2_1)) ==> QPMask[null, Q(r_2_1)] == Mask[null, Q(r_2_1)]
+      );
+    
+    // -- assume permission updates for independent locations 
+      assume (forall <A, B> o_2: Ref, f_4: (Field A B) ::
+        { Mask[o_2, f_4] } { QPMask[o_2, f_4] }
+        (o_2 != null || !IsPredicateField(f_4)) || getPredicateId(f_4) != 4 ==> Mask[o_2, f_4] == QPMask[o_2, f_4]
+      );
+    Mask := QPMask;
+    havoc wildcard;
+    perm := wildcard;
+    Mask[null, P2(r_1)] := Mask[null, P2(r_1)] + perm;
+    assume state(Heap, Mask);
+    assume state(Heap, Mask);
+    assume P2#trigger(Heap, P2(r_1));
+    assume Heap[null, P2(r_1)] == FrameFragment(P2#condqp2(Heap, r_1));
+    if (!HasDirectPerm(Mask, null, P2(r_1))) {
+      Heap[null, P2#sm(r_1)] := ZeroPMask;
+      havoc freshVersion;
+      Heap[null, P2(r_1)] := freshVersion;
+    }
+    assume state(Heap, Mask);
+    assume state(Heap, Mask);
+  
+  // -- Translating statement: unfold acc(P2(r), wildcard) -- 0196.vpr@67.18--68.5
+    assume P2#trigger(Heap, P2(r_1));
+    assume Heap[null, P2(r_1)] == FrameFragment(P2#condqp2(Heap, r_1));
+    // Phase 1: pure assertions and fixed permissions
+    
+    // -- Update version of predicate
+      if (!HasDirectPerm(Mask, null, P2(r_1))) {
+        havoc newVersion;
+        Heap[null, P2(r_1)] := newVersion;
+      }
+    // Phase 3: all remaining permissions (containing read permissions, but in a negative context)
+    perm := NoPerm;
+    havoc wildcard;
+    perm := perm + wildcard;
+    assert {:msg "  Unfolding P2(r) might fail. There might be insufficient permission to access P2(r) (0196.vpr@67.18--68.5) [150]"}
+      Mask[null, P2(r_1)] > NoPerm;
+    assume wildcard < Mask[null, P2(r_1)];
+    Mask[null, P2(r_1)] := Mask[null, P2(r_1)] - perm;
+    assume state(Heap, Mask);
+    havoc QPMask;
+    havoc wildcard;
+    
+    // -- Define Inverse Function
+      assume (forall e_3: Ref ::
+        { Heap[null, Q(e_3)] } { Mask[null, Q(e_3)] } { refs(Heap, r_1)[e_3] }
+        refs(Heap, r_1)[e_3] && NoPerm < wildcard ==> invRecv12(e_3) == e_3 && qpRange12(e_3)
+      );
+      assume (forall r_3_1: Ref ::
+        { invRecv12(r_3_1) }
+        (refs(Heap, r_1)[invRecv12(r_3_1)] && NoPerm < wildcard) && qpRange12(r_3_1) ==> invRecv12(r_3_1) == r_3_1
+      );
+    // Assume permission expression is non-negative for all fields
+    assume (forall e_3: Ref ::
+      { Heap[null, Q(e_3)] } { Mask[null, Q(e_3)] } { refs(Heap, r_1)[e_3] }
+      refs(Heap, r_1)[e_3] ==> wildcard >= NoPerm
+    );
+    
+    // -- Define updated permissions
+      assume (forall r_3_1: Ref ::
+        { QPMask[null, Q(r_3_1)] }
+        (refs(Heap, r_1)[invRecv12(r_3_1)] && NoPerm < wildcard) && qpRange12(r_3_1) ==> (NoPerm < wildcard ==> invRecv12(r_3_1) == r_3_1) && QPMask[null, Q(r_3_1)] == Mask[null, Q(r_3_1)] + wildcard
+      );
+    
+    // -- Define independent locations
+      assume (forall <A, B> o_2: Ref, f_4: (Field A B) ::
+        { Mask[o_2, f_4] } { QPMask[o_2, f_4] }
+        (o_2 != null || !IsPredicateField(f_4)) || getPredicateId(f_4) != 4 ==> Mask[o_2, f_4] == QPMask[o_2, f_4]
+      );
+      assume (forall r_3_1: Ref ::
+        { QPMask[null, Q(r_3_1)] }
+        !((refs(Heap, r_1)[invRecv12(r_3_1)] && NoPerm < wildcard) && qpRange12(r_3_1)) ==> QPMask[null, Q(r_3_1)] == Mask[null, Q(r_3_1)]
+      );
+    Mask := QPMask;
+    assume state(Heap, Mask);
+    assume state(Heap, Mask);
+    assume state(Heap, Mask);
+  
+  // -- Translating statement: r2 := tester(get(r)) -- 0196.vpr@68.8--71.1
+    
+    // -- Check definedness of tester(get(r))
+      if (*) {
+        // Stop execution
+        assume false;
+      }
+      if (*) {
+        // Exhale precondition of function application
+        // Phase 3: all remaining permissions (containing read permissions, but in a negative context)
+        perm := NoPerm;
+        havoc wildcard;
+        perm := perm + wildcard;
+        assert {:msg "  Precondition of function tester might not hold. There might be insufficient permission to access Q(get(r)) (0196.vpr@68.27--68.27) [151]"}
+          Mask[null, Q(get(Heap, r_1))] > NoPerm;
+        assume wildcard < Mask[null, Q(get(Heap, r_1))];
+        Mask[null, Q(get(Heap, r_1))] := Mask[null, Q(get(Heap, r_1))] - perm;
+        // Finish exhale
+        havoc ExhaleHeap;
+        assume IdenticalOnKnownLocations(Heap, ExhaleHeap, Mask);
+        Heap := ExhaleHeap;
+        // Stop execution
+        assume false;
+      }
+      assume state(Heap, Mask);
+    r2 := tester(Heap, get(Heap, r_1));
+    assume state(Heap, Mask);
+}
+
+// ==================================================
+// Translation of method func1
+// ==================================================
+
+procedure func1(r_1: Ref) returns ()
+  modifies Heap, Mask;
+{
+  var wildcard: real where wildcard > NoPerm;
+  var perm: Perm;
+  var r2: Ref;
+  var newVersion: FrameType;
+  var QPMask: MaskType;
+  var freshVersion: FrameType;
+  var newPMask: PMaskType;
+  var ExhaleHeap: HeapType;
+  
+  // -- Initializing the state
+    Mask := ZeroMask;
+    assume state(Heap, Mask);
+    assume AssumeFunctionsAbove == -1;
+  
+  // -- Assumptions about method arguments
+    assume Heap[r_1, $allocated];
+  
+  // -- Checked inhaling of precondition
+    havoc wildcard;
+    perm := wildcard;
+    Mask[null, R(r_1)] := Mask[null, R(r_1)] + perm;
+    assume state(Heap, Mask);
+    assume state(Heap, Mask);
+  
+  // -- Initializing of old state
+    
+    // -- Initializing the old state
+      assume Heap == old(Heap);
+      assume Mask == old(Mask);
+  
+  // -- Assumptions about local variables
+    assume Heap[r2, $allocated];
+  
+  // -- Translating statement: unfold acc(R(r), wildcard) -- 0196.vpr@76.17--77.5
+    assume R#trigger(Heap, R(r_1));
+    assume Heap[null, R(r_1)] == FrameFragment(R#condqp3(Heap, r_1));
+    // Phase 1: pure assertions and fixed permissions
+    
+    // -- Update version of predicate
+      if (!HasDirectPerm(Mask, null, R(r_1))) {
+        havoc newVersion;
+        Heap[null, R(r_1)] := newVersion;
+      }
+    // Phase 3: all remaining permissions (containing read permissions, but in a negative context)
+    perm := NoPerm;
+    havoc wildcard;
+    perm := perm + wildcard;
+    assert {:msg "  Unfolding R(r) might fail. There might be insufficient permission to access R(r) (0196.vpr@76.17--77.5) [152]"}
+      Mask[null, R(r_1)] > NoPerm;
+    assume wildcard < Mask[null, R(r_1)];
+    Mask[null, R(r_1)] := Mask[null, R(r_1)] - perm;
+    assume state(Heap, Mask);
+    havoc QPMask;
+    havoc wildcard;
+    
+    // -- Define Inverse Function
+      assume (forall e: Ref ::
+        { Heap[e, q_1] } { QPMask[e, q_1] } { refs(Heap, r_1)[e] }
+        refs(Heap, r_1)[e] && NoPerm < wildcard ==> qpRange13(e) && invRecv13(e) == e
+      );
       assume (forall o_2: Ref ::
-        { QPMask[o_2, f_6] } { QPBMask[o_2, f_6] }
-        (s[invRecv2(o_2)] && qpRange2(o_2) ==> invRecv2(o_2) == o_2 && (QPMask[o_2, f_6] == Mask[o_2, f_6] && QPBMask[o_2, f_6] == BMask[o_2, f_6])) && (!(s[invRecv2(o_2)] && qpRange2(o_2)) ==> QPMask[o_2, f_6] == Mask[o_2, f_6] && QPBMask[o_2, f_6] == BMask[o_2, f_6])
+        { invRecv13(o_2) }
+        (refs(Heap, r_1)[invRecv13(o_2)] && NoPerm < wildcard) && qpRange13(o_2) ==> invRecv13(o_2) == o_2
+      );
+    
+    // -- Assume set of fields is nonNull
+      assume (forall e: Ref ::
+        { Heap[e, q_1] } { QPMask[e, q_1] } { refs(Heap, r_1)[e] }
+        refs(Heap, r_1)[e] && wildcard > NoPerm ==> e != null
+      );
+    // Assume permission expression is non-negative for all fields
+    assume (forall e: Ref ::
+      { Heap[e, q_1] } { QPMask[e, q_1] } { refs(Heap, r_1)[e] }
+      refs(Heap, r_1)[e] ==> wildcard >= NoPerm
+    );
+    
+    // -- Define permissions
+      assume (forall o_2: Ref ::
+        { QPMask[o_2, q_1] }
+        ((refs(Heap, r_1)[invRecv13(o_2)] && NoPerm < wildcard) && qpRange13(o_2) ==> (NoPerm < wildcard ==> invRecv13(o_2) == o_2) && QPMask[o_2, q_1] == Mask[o_2, q_1] + wildcard) && (!((refs(Heap, r_1)[invRecv13(o_2)] && NoPerm < wildcard) && qpRange13(o_2)) ==> QPMask[o_2, q_1] == Mask[o_2, q_1])
+      );
+      assume (forall <A, B> o_2: Ref, f_4: (Field A B) ::
+        { Mask[o_2, f_4] } { QPMask[o_2, f_4] }
+        f_4 != q_1 ==> Mask[o_2, f_4] == QPMask[o_2, f_4]
+      );
+    Mask := QPMask;
+    assume state(Heap, Mask);
+    assume state(Heap, Mask);
+    assume state(Heap, Mask);
+  
+  // -- Translating statement: fold acc(R(r), wildcard) -- 0196.vpr@77.15--78.5
+    // Phase 1: pure assertions and fixed permissions
+    havoc QPMask;
+    // wild card assumptions
+    havoc wildcard;
+    assert {:msg "  Folding R(r) might fail. There might be insufficient permission to access e.q (0196.vpr@77.15--78.5) [153]"}
+      (forall e_1: Ref ::
+      
+      refs(Heap, r_1)[e_1] ==> Mask[e_1, q_1] > NoPerm
+    );
+    assume (forall e_1: Ref ::
+      
+      refs(Heap, r_1)[e_1] ==> wildcard < Mask[e_1, q_1]
+    );
+    
+    // -- check that the permission amount is positive
+      assert {:msg "  Folding R(r) might fail. Fraction wildcard * wildcard might be negative. (0196.vpr@77.15--78.5) [154]"}
+        (forall e_1: Ref ::
+        { Heap[e_1, q_1] } { QPMask[e_1, q_1] } { refs(Heap, r_1)[e_1] }
+        refs(Heap, r_1)[e_1] && dummyFunction(Heap[e_1, q_1]) ==> wildcard >= NoPerm
+      );
+    
+    // -- check if receiver e is injective
+      assert {:msg "  Folding R(r) might fail. Receiver of e.q [0196.vpr@6.64--6.64]  might not be injective. (0196.vpr@77.15--78.5) [155]"}
+        (forall e_1: Ref, e_1_1: Ref ::
+        { neverTriggered14(e_1), neverTriggered14(e_1_1) }
+        (((e_1 != e_1_1 && refs(Heap, r_1)[e_1]) && refs(Heap, r_1)[e_1_1]) && NoPerm < wildcard) && NoPerm < wildcard ==> e_1 != e_1_1
+      );
+    
+    // -- check if sufficient permission is held
+      assert {:msg "  Folding R(r) might fail. There might be insufficient permission to access e.q (0196.vpr@77.15--78.5) [156]"}
+        (forall e_1: Ref ::
+        { Heap[e_1, q_1] } { QPMask[e_1, q_1] } { refs(Heap, r_1)[e_1] }
+        refs(Heap, r_1)[e_1] ==> Mask[e_1, q_1] > NoPerm
+      );
+    
+    // -- assumptions for inverse of receiver e
+      assume (forall e_1: Ref ::
+        { Heap[e_1, q_1] } { QPMask[e_1, q_1] } { refs(Heap, r_1)[e_1] }
+        refs(Heap, r_1)[e_1] && NoPerm < wildcard ==> qpRange14(e_1) && invRecv14(e_1) == e_1
+      );
+      assume (forall o_2: Ref ::
+        { invRecv14(o_2) }
+        refs(Heap, r_1)[invRecv14(o_2)] && (NoPerm < wildcard && qpRange14(o_2)) ==> invRecv14(o_2) == o_2
+      );
+    
+    // -- assume permission updates for field q
+      assume (forall o_2: Ref ::
+        { QPMask[o_2, q_1] }
+        (refs(Heap, r_1)[invRecv14(o_2)] && (NoPerm < wildcard && qpRange14(o_2)) ==> invRecv14(o_2) == o_2 && QPMask[o_2, q_1] == Mask[o_2, q_1] - wildcard) && (!(refs(Heap, r_1)[invRecv14(o_2)] && (NoPerm < wildcard && qpRange14(o_2))) ==> QPMask[o_2, q_1] == Mask[o_2, q_1])
       );
     
     // -- assume permission updates for independent locations
       assume (forall <A, B> o_2: Ref, f_4: (Field A B) ::
-        { QPMask[o_2, f_4] } { QPBMask[o_2, f_4] }
-        f_4 != f_6 ==> Mask[o_2, f_4] == QPMask[o_2, f_4] && BMask[o_2, f_4] == QPBMask[o_2, f_4]
+        { QPMask[o_2, f_4] }
+        f_4 != q_1 ==> Mask[o_2, f_4] == QPMask[o_2, f_4]
       );
     Mask := QPMask;
-    BMask := QPBMask;
-    // Finish exhale
-    havoc ExhaleHeap;
-    assume IdenticalOnKnownLocations(Heap, ExhaleHeap, Mask, BMask);
-    Heap := ExhaleHeap;
-    assume state(Heap, Mask, BMask);
+    havoc wildcard;
+    perm := wildcard;
+    Mask[null, R(r_1)] := Mask[null, R(r_1)] + perm;
+    assume state(Heap, Mask);
+    assume state(Heap, Mask);
+    assume R#trigger(Heap, R(r_1));
+    assume Heap[null, R(r_1)] == FrameFragment(R#condqp3(Heap, r_1));
+    if (!HasDirectPerm(Mask, null, R(r_1))) {
+      Heap[null, R#sm(r_1)] := ZeroPMask;
+      havoc freshVersion;
+      Heap[null, R(r_1)] := freshVersion;
+    }
+    // register all known folded permissions guarded by predicate R
+    havoc newPMask;
+    assume (forall <A, B> o_3: Ref, f_6: (Field A B) ::
+      { newPMask[o_3, f_6] }
+      Heap[null, R#sm(r_1)][o_3, f_6] ==> newPMask[o_3, f_6]
+    );
+    assume (forall e_2: Ref ::
+      
+      refs(Heap, r_1)[e_2] ==> newPMask[e_2, q_1]
+    );
+    Heap[null, R#sm(r_1)] := newPMask;
+    assume state(Heap, Mask);
+    assume state(Heap, Mask);
+  
+  // -- Translating statement: unfold acc(R(r), wildcard) -- 0196.vpr@78.17--79.5
+    assume R#trigger(Heap, R(r_1));
+    assume Heap[null, R(r_1)] == FrameFragment(R#condqp3(Heap, r_1));
+    // Phase 1: pure assertions and fixed permissions
+    
+    // -- Update version of predicate
+      if (!HasDirectPerm(Mask, null, R(r_1))) {
+        havoc newVersion;
+        Heap[null, R(r_1)] := newVersion;
+      }
+    // Phase 3: all remaining permissions (containing read permissions, but in a negative context)
+    perm := NoPerm;
+    havoc wildcard;
+    perm := perm + wildcard;
+    assert {:msg "  Unfolding R(r) might fail. There might be insufficient permission to access R(r) (0196.vpr@78.17--79.5) [157]"}
+      Mask[null, R(r_1)] > NoPerm;
+    assume wildcard < Mask[null, R(r_1)];
+    Mask[null, R(r_1)] := Mask[null, R(r_1)] - perm;
+    assume state(Heap, Mask);
+    havoc QPMask;
+    havoc wildcard;
+    
+    // -- Define Inverse Function
+      assume (forall e_3: Ref ::
+        { Heap[e_3, q_1] } { QPMask[e_3, q_1] } { refs(Heap, r_1)[e_3] }
+        refs(Heap, r_1)[e_3] && NoPerm < wildcard ==> qpRange15(e_3) && invRecv15(e_3) == e_3
+      );
+      assume (forall o_2: Ref ::
+        { invRecv15(o_2) }
+        (refs(Heap, r_1)[invRecv15(o_2)] && NoPerm < wildcard) && qpRange15(o_2) ==> invRecv15(o_2) == o_2
+      );
+    
+    // -- Assume set of fields is nonNull
+      assume (forall e_3: Ref ::
+        { Heap[e_3, q_1] } { QPMask[e_3, q_1] } { refs(Heap, r_1)[e_3] }
+        refs(Heap, r_1)[e_3] && wildcard > NoPerm ==> e_3 != null
+      );
+    // Assume permission expression is non-negative for all fields
+    assume (forall e_3: Ref ::
+      { Heap[e_3, q_1] } { QPMask[e_3, q_1] } { refs(Heap, r_1)[e_3] }
+      refs(Heap, r_1)[e_3] ==> wildcard >= NoPerm
+    );
+    
+    // -- Define permissions
+      assume (forall o_2: Ref ::
+        { QPMask[o_2, q_1] }
+        ((refs(Heap, r_1)[invRecv15(o_2)] && NoPerm < wildcard) && qpRange15(o_2) ==> (NoPerm < wildcard ==> invRecv15(o_2) == o_2) && QPMask[o_2, q_1] == Mask[o_2, q_1] + wildcard) && (!((refs(Heap, r_1)[invRecv15(o_2)] && NoPerm < wildcard) && qpRange15(o_2)) ==> QPMask[o_2, q_1] == Mask[o_2, q_1])
+      );
+      assume (forall <A, B> o_2: Ref, f_4: (Field A B) ::
+        { Mask[o_2, f_4] } { QPMask[o_2, f_4] }
+        f_4 != q_1 ==> Mask[o_2, f_4] == QPMask[o_2, f_4]
+      );
+    Mask := QPMask;
+    assume state(Heap, Mask);
+    assume state(Heap, Mask);
+    assume state(Heap, Mask);
+  
+  // -- Translating statement: r2 := testerfield(get(r)) -- 0196.vpr@79.8--82.1
+    
+    // -- Check definedness of testerfield(get(r))
+      if (*) {
+        // Stop execution
+        assume false;
+      }
+      if (*) {
+        // Exhale precondition of function application
+        // Phase 3: all remaining permissions (containing read permissions, but in a negative context)
+        perm := NoPerm;
+        havoc wildcard;
+        perm := perm + wildcard;
+        assert {:msg "  Precondition of function testerfield might not hold. There might be insufficient permission to access get(r).q (0196.vpr@79.32--79.32) [158]"}
+          Mask[get(Heap, r_1), q_1] > NoPerm;
+        assume wildcard < Mask[get(Heap, r_1), q_1];
+        Mask[get(Heap, r_1), q_1] := Mask[get(Heap, r_1), q_1] - perm;
+        // Finish exhale
+        havoc ExhaleHeap;
+        assume IdenticalOnKnownLocations(Heap, ExhaleHeap, Mask);
+        Heap := ExhaleHeap;
+        // Stop execution
+        assume false;
+      }
+      assume state(Heap, Mask);
+    r2 := testerfield(Heap, get(Heap, r_1));
+    assume state(Heap, Mask);
+}
+
+// ==================================================
+// Translation of method func2
+// ==================================================
+
+procedure func2(r_1: Ref) returns ()
+  modifies Heap, Mask;
+{
+  var perm: Perm;
+  var r2: Ref;
+  var newVersion: FrameType;
+  var QPMask: MaskType;
+  var wildcard: real where wildcard > NoPerm;
+  var freshVersion: FrameType;
+  var newPMask: PMaskType;
+  var ExhaleHeap: HeapType;
+  
+  // -- Initializing the state
+    Mask := ZeroMask;
+    assume state(Heap, Mask);
+    assume AssumeFunctionsAbove == -1;
+  
+  // -- Assumptions about method arguments
+    assume Heap[r_1, $allocated];
+  
+  // -- Checked inhaling of precondition
+    perm := FullPerm;
+    Mask[null, R(r_1)] := Mask[null, R(r_1)] + perm;
+    assume state(Heap, Mask);
+    assume state(Heap, Mask);
+  
+  // -- Initializing of old state
+    
+    // -- Initializing the old state
+      assume Heap == old(Heap);
+      assume Mask == old(Mask);
+  
+  // -- Assumptions about local variables
+    assume Heap[r2, $allocated];
+  
+  // -- Translating statement: unfold acc(R(r), write) -- 0196.vpr@87.17--88.5
+    assume R#trigger(Heap, R(r_1));
+    assume Heap[null, R(r_1)] == FrameFragment(R#condqp3(Heap, r_1));
+    // Phase 1: pure assertions and fixed permissions
+    perm := NoPerm;
+    perm := perm + FullPerm;
+    if (perm != NoPerm) {
+      assert {:msg "  Unfolding R(r) might fail. There might be insufficient permission to access R(r) (0196.vpr@87.17--88.5) [160]"}
+        perm <= Mask[null, R(r_1)];
+    }
+    Mask[null, R(r_1)] := Mask[null, R(r_1)] - perm;
+    
+    // -- Update version of predicate
+      if (!HasDirectPerm(Mask, null, R(r_1))) {
+        havoc newVersion;
+        Heap[null, R(r_1)] := newVersion;
+      }
+    assume state(Heap, Mask);
+    havoc QPMask;
+    havoc wildcard;
+    
+    // -- Define Inverse Function
+      assume (forall e: Ref ::
+        { Heap[e, q_1] } { QPMask[e, q_1] } { refs(Heap, r_1)[e] }
+        refs(Heap, r_1)[e] && NoPerm < wildcard ==> qpRange16(e) && invRecv16(e) == e
+      );
+      assume (forall o_2: Ref ::
+        { invRecv16(o_2) }
+        (refs(Heap, r_1)[invRecv16(o_2)] && NoPerm < wildcard) && qpRange16(o_2) ==> invRecv16(o_2) == o_2
+      );
+    
+    // -- Assume set of fields is nonNull
+      assume (forall e: Ref ::
+        { Heap[e, q_1] } { QPMask[e, q_1] } { refs(Heap, r_1)[e] }
+        refs(Heap, r_1)[e] ==> e != null
+      );
+    // Assume permission expression is non-negative for all fields
+    assume (forall e: Ref ::
+      { Heap[e, q_1] } { QPMask[e, q_1] } { refs(Heap, r_1)[e] }
+      refs(Heap, r_1)[e] ==> wildcard >= NoPerm
+    );
+    
+    // -- Define permissions
+      assume (forall o_2: Ref ::
+        { QPMask[o_2, q_1] }
+        ((refs(Heap, r_1)[invRecv16(o_2)] && NoPerm < wildcard) && qpRange16(o_2) ==> (NoPerm < wildcard ==> invRecv16(o_2) == o_2) && QPMask[o_2, q_1] == Mask[o_2, q_1] + wildcard) && (!((refs(Heap, r_1)[invRecv16(o_2)] && NoPerm < wildcard) && qpRange16(o_2)) ==> QPMask[o_2, q_1] == Mask[o_2, q_1])
+      );
+      assume (forall <A, B> o_2: Ref, f_4: (Field A B) ::
+        { Mask[o_2, f_4] } { QPMask[o_2, f_4] }
+        f_4 != q_1 ==> Mask[o_2, f_4] == QPMask[o_2, f_4]
+      );
+    Mask := QPMask;
+    assume state(Heap, Mask);
+    assume state(Heap, Mask);
+    assume state(Heap, Mask);
+  
+  // -- Translating statement: fold acc(R(r), write) -- 0196.vpr@88.15--89.5
+    // Phase 1: pure assertions and fixed permissions
+    havoc QPMask;
+    // wild card assumptions
+    havoc wildcard;
+    assert {:msg "  Folding R(r) might fail. There might be insufficient permission to access e.q (0196.vpr@88.15--89.5) [161]"}
+      (forall e_1: Ref ::
+      
+      refs(Heap, r_1)[e_1] ==> Mask[e_1, q_1] > NoPerm
+    );
+    assume (forall e_1: Ref ::
+      
+      refs(Heap, r_1)[e_1] ==> wildcard < Mask[e_1, q_1]
+    );
+    
+    // -- check that the permission amount is positive
+      assert {:msg "  Folding R(r) might fail. Fraction wildcard might be negative. (0196.vpr@88.15--89.5) [162]"}
+        (forall e_1: Ref ::
+        { Heap[e_1, q_1] } { QPMask[e_1, q_1] } { refs(Heap, r_1)[e_1] }
+        refs(Heap, r_1)[e_1] && dummyFunction(Heap[e_1, q_1]) ==> wildcard >= NoPerm
+      );
+    
+    // -- check if receiver e is injective
+      assert {:msg "  Folding R(r) might fail. Receiver of e.q [0196.vpr@6.64--6.64]  might not be injective. (0196.vpr@88.15--89.5) [163]"}
+        (forall e_1: Ref, e_1_1: Ref ::
+        { neverTriggered17(e_1), neverTriggered17(e_1_1) }
+        (((e_1 != e_1_1 && refs(Heap, r_1)[e_1]) && refs(Heap, r_1)[e_1_1]) && NoPerm < wildcard) && NoPerm < wildcard ==> e_1 != e_1_1
+      );
+    
+    // -- check if sufficient permission is held
+      assert {:msg "  Folding R(r) might fail. There might be insufficient permission to access e.q (0196.vpr@88.15--89.5) [164]"}
+        (forall e_1: Ref ::
+        { Heap[e_1, q_1] } { QPMask[e_1, q_1] } { refs(Heap, r_1)[e_1] }
+        refs(Heap, r_1)[e_1] ==> Mask[e_1, q_1] > NoPerm
+      );
+    
+    // -- assumptions for inverse of receiver e
+      assume (forall e_1: Ref ::
+        { Heap[e_1, q_1] } { QPMask[e_1, q_1] } { refs(Heap, r_1)[e_1] }
+        refs(Heap, r_1)[e_1] && NoPerm < wildcard ==> qpRange17(e_1) && invRecv17(e_1) == e_1
+      );
+      assume (forall o_2: Ref ::
+        { invRecv17(o_2) }
+        refs(Heap, r_1)[invRecv17(o_2)] && (NoPerm < wildcard && qpRange17(o_2)) ==> invRecv17(o_2) == o_2
+      );
+    
+    // -- assume permission updates for field q
+      assume (forall o_2: Ref ::
+        { QPMask[o_2, q_1] }
+        (refs(Heap, r_1)[invRecv17(o_2)] && (NoPerm < wildcard && qpRange17(o_2)) ==> invRecv17(o_2) == o_2 && QPMask[o_2, q_1] == Mask[o_2, q_1] - wildcard) && (!(refs(Heap, r_1)[invRecv17(o_2)] && (NoPerm < wildcard && qpRange17(o_2))) ==> QPMask[o_2, q_1] == Mask[o_2, q_1])
+      );
+    
+    // -- assume permission updates for independent locations
+      assume (forall <A, B> o_2: Ref, f_4: (Field A B) ::
+        { QPMask[o_2, f_4] }
+        f_4 != q_1 ==> Mask[o_2, f_4] == QPMask[o_2, f_4]
+      );
+    Mask := QPMask;
+    perm := FullPerm;
+    Mask[null, R(r_1)] := Mask[null, R(r_1)] + perm;
+    assume state(Heap, Mask);
+    assume state(Heap, Mask);
+    assume R#trigger(Heap, R(r_1));
+    assume Heap[null, R(r_1)] == FrameFragment(R#condqp3(Heap, r_1));
+    if (!HasDirectPerm(Mask, null, R(r_1))) {
+      Heap[null, R#sm(r_1)] := ZeroPMask;
+      havoc freshVersion;
+      Heap[null, R(r_1)] := freshVersion;
+    }
+    // register all known folded permissions guarded by predicate R
+    havoc newPMask;
+    assume (forall <A, B> o_4: Ref, f_7: (Field A B) ::
+      { newPMask[o_4, f_7] }
+      Heap[null, R#sm(r_1)][o_4, f_7] ==> newPMask[o_4, f_7]
+    );
+    assume (forall e_2: Ref ::
+      
+      refs(Heap, r_1)[e_2] ==> newPMask[e_2, q_1]
+    );
+    Heap[null, R#sm(r_1)] := newPMask;
+    assume state(Heap, Mask);
+    assume state(Heap, Mask);
+  
+  // -- Translating statement: unfold acc(R(r), write) -- 0196.vpr@89.17--90.5
+    assume R#trigger(Heap, R(r_1));
+    assume Heap[null, R(r_1)] == FrameFragment(R#condqp3(Heap, r_1));
+    // Phase 1: pure assertions and fixed permissions
+    perm := NoPerm;
+    perm := perm + FullPerm;
+    if (perm != NoPerm) {
+      assert {:msg "  Unfolding R(r) might fail. There might be insufficient permission to access R(r) (0196.vpr@89.17--90.5) [166]"}
+        perm <= Mask[null, R(r_1)];
+    }
+    Mask[null, R(r_1)] := Mask[null, R(r_1)] - perm;
+    
+    // -- Update version of predicate
+      if (!HasDirectPerm(Mask, null, R(r_1))) {
+        havoc newVersion;
+        Heap[null, R(r_1)] := newVersion;
+      }
+    assume state(Heap, Mask);
+    havoc QPMask;
+    havoc wildcard;
+    
+    // -- Define Inverse Function
+      assume (forall e_3: Ref ::
+        { Heap[e_3, q_1] } { QPMask[e_3, q_1] } { refs(Heap, r_1)[e_3] }
+        refs(Heap, r_1)[e_3] && NoPerm < wildcard ==> qpRange18(e_3) && invRecv18(e_3) == e_3
+      );
+      assume (forall o_2: Ref ::
+        { invRecv18(o_2) }
+        (refs(Heap, r_1)[invRecv18(o_2)] && NoPerm < wildcard) && qpRange18(o_2) ==> invRecv18(o_2) == o_2
+      );
+    
+    // -- Assume set of fields is nonNull
+      assume (forall e_3: Ref ::
+        { Heap[e_3, q_1] } { QPMask[e_3, q_1] } { refs(Heap, r_1)[e_3] }
+        refs(Heap, r_1)[e_3] ==> e_3 != null
+      );
+    // Assume permission expression is non-negative for all fields
+    assume (forall e_3: Ref ::
+      { Heap[e_3, q_1] } { QPMask[e_3, q_1] } { refs(Heap, r_1)[e_3] }
+      refs(Heap, r_1)[e_3] ==> wildcard >= NoPerm
+    );
+    
+    // -- Define permissions
+      assume (forall o_2: Ref ::
+        { QPMask[o_2, q_1] }
+        ((refs(Heap, r_1)[invRecv18(o_2)] && NoPerm < wildcard) && qpRange18(o_2) ==> (NoPerm < wildcard ==> invRecv18(o_2) == o_2) && QPMask[o_2, q_1] == Mask[o_2, q_1] + wildcard) && (!((refs(Heap, r_1)[invRecv18(o_2)] && NoPerm < wildcard) && qpRange18(o_2)) ==> QPMask[o_2, q_1] == Mask[o_2, q_1])
+      );
+      assume (forall <A, B> o_2: Ref, f_4: (Field A B) ::
+        { Mask[o_2, f_4] } { QPMask[o_2, f_4] }
+        f_4 != q_1 ==> Mask[o_2, f_4] == QPMask[o_2, f_4]
+      );
+    Mask := QPMask;
+    assume state(Heap, Mask);
+    assume state(Heap, Mask);
+    assume state(Heap, Mask);
+  
+  // -- Translating statement: r2 := testerfield(get(r)) -- 0196.vpr@90.8--93.1
+    
+    // -- Check definedness of testerfield(get(r))
+      if (*) {
+        // Stop execution
+        assume false;
+      }
+      if (*) {
+        // Exhale precondition of function application
+        // Phase 3: all remaining permissions (containing read permissions, but in a negative context)
+        perm := NoPerm;
+        havoc wildcard;
+        perm := perm + wildcard;
+        assert {:msg "  Precondition of function testerfield might not hold. There might be insufficient permission to access get(r).q (0196.vpr@90.32--90.32) [167]"}
+          Mask[get(Heap, r_1), q_1] > NoPerm;
+        assume wildcard < Mask[get(Heap, r_1), q_1];
+        Mask[get(Heap, r_1), q_1] := Mask[get(Heap, r_1), q_1] - perm;
+        // Finish exhale
+        havoc ExhaleHeap;
+        assume IdenticalOnKnownLocations(Heap, ExhaleHeap, Mask);
+        Heap := ExhaleHeap;
+        // Stop execution
+        assume false;
+      }
+      assume state(Heap, Mask);
+    r2 := testerfield(Heap, get(Heap, r_1));
+    assume state(Heap, Mask);
+}
+
+// ==================================================
+// Translation of method func3
+// ==================================================
+
+procedure func3(r_1: Ref) returns ()
+  modifies Heap, Mask;
+{
+  var perm: Perm;
+  var r2: Ref;
+  var newVersion: FrameType;
+  var QPMask: MaskType;
+  var wildcard: real where wildcard > NoPerm;
+  var freshVersion: FrameType;
+  var newPMask: PMaskType;
+  var ExhaleHeap: HeapType;
+  
+  // -- Initializing the state
+    Mask := ZeroMask;
+    assume state(Heap, Mask);
+    assume AssumeFunctionsAbove == -1;
+  
+  // -- Assumptions about method arguments
+    assume Heap[r_1, $allocated];
+  
+  // -- Checked inhaling of precondition
+    perm := FullPerm;
+    Mask[null, R(r_1)] := Mask[null, R(r_1)] + perm;
+    assume state(Heap, Mask);
+    assume state(Heap, Mask);
+  
+  // -- Initializing of old state
+    
+    // -- Initializing the old state
+      assume Heap == old(Heap);
+      assume Mask == old(Mask);
+  
+  // -- Assumptions about local variables
+    assume Heap[r2, $allocated];
+  
+  // -- Translating statement: unfold acc(R(r), 1 / 2) -- 0196.vpr@98.17--99.5
+    assume R#trigger(Heap, R(r_1));
+    assume Heap[null, R(r_1)] == FrameFragment(R#condqp3(Heap, r_1));
+    // Phase 1: pure assertions and fixed permissions
+    assert {:msg "  Unfolding R(r) might fail. Fraction 1 / 2 might be negative. (0196.vpr@98.17--99.5) [168]"}
+      1 / 2 >= NoPerm;
+    perm := NoPerm;
+    perm := perm + 1 / 2;
+    if (perm != NoPerm) {
+      assert {:msg "  Unfolding R(r) might fail. There might be insufficient permission to access R(r) (0196.vpr@98.17--99.5) [169]"}
+        perm <= Mask[null, R(r_1)];
+    }
+    Mask[null, R(r_1)] := Mask[null, R(r_1)] - perm;
+    
+    // -- Update version of predicate
+      if (!HasDirectPerm(Mask, null, R(r_1))) {
+        havoc newVersion;
+        Heap[null, R(r_1)] := newVersion;
+      }
+    assume state(Heap, Mask);
+    havoc QPMask;
+    havoc wildcard;
+    
+    // -- Define Inverse Function
+      assume (forall e: Ref ::
+        { Heap[e, q_1] } { QPMask[e, q_1] } { refs(Heap, r_1)[e] }
+        refs(Heap, r_1)[e] && NoPerm < wildcard ==> qpRange19(e) && invRecv19(e) == e
+      );
+      assume (forall o_2: Ref ::
+        { invRecv19(o_2) }
+        (refs(Heap, r_1)[invRecv19(o_2)] && NoPerm < wildcard) && qpRange19(o_2) ==> invRecv19(o_2) == o_2
+      );
+    
+    // -- Assume set of fields is nonNull
+      assume (forall e: Ref ::
+        { Heap[e, q_1] } { QPMask[e, q_1] } { refs(Heap, r_1)[e] }
+        refs(Heap, r_1)[e] && wildcard > NoPerm ==> e != null
+      );
+    // Assume permission expression is non-negative for all fields
+    assume (forall e: Ref ::
+      { Heap[e, q_1] } { QPMask[e, q_1] } { refs(Heap, r_1)[e] }
+      refs(Heap, r_1)[e] ==> wildcard >= NoPerm
+    );
+    
+    // -- Define permissions
+      assume (forall o_2: Ref ::
+        { QPMask[o_2, q_1] }
+        ((refs(Heap, r_1)[invRecv19(o_2)] && NoPerm < wildcard) && qpRange19(o_2) ==> (NoPerm < wildcard ==> invRecv19(o_2) == o_2) && QPMask[o_2, q_1] == Mask[o_2, q_1] + wildcard) && (!((refs(Heap, r_1)[invRecv19(o_2)] && NoPerm < wildcard) && qpRange19(o_2)) ==> QPMask[o_2, q_1] == Mask[o_2, q_1])
+      );
+      assume (forall <A, B> o_2: Ref, f_4: (Field A B) ::
+        { Mask[o_2, f_4] } { QPMask[o_2, f_4] }
+        f_4 != q_1 ==> Mask[o_2, f_4] == QPMask[o_2, f_4]
+      );
+    Mask := QPMask;
+    assume state(Heap, Mask);
+    assume state(Heap, Mask);
+    assume state(Heap, Mask);
+  
+  // -- Translating statement: fold acc(R(r), 1 / 2) -- 0196.vpr@99.15--100.5
+    // Phase 1: pure assertions and fixed permissions
+    havoc QPMask;
+    // wild card assumptions
+    havoc wildcard;
+    assert {:msg "  Folding R(r) might fail. There might be insufficient permission to access e.q (0196.vpr@99.15--100.5) [170]"}
+      (forall e_1: Ref ::
+      
+      refs(Heap, r_1)[e_1] ==> Mask[e_1, q_1] > NoPerm
+    );
+    assume (forall e_1: Ref ::
+      
+      refs(Heap, r_1)[e_1] ==> wildcard < Mask[e_1, q_1]
+    );
+    
+    // -- check that the permission amount is positive
+      assert {:msg "  Folding R(r) might fail. Fraction wildcard * (1 / 2) might be negative. (0196.vpr@99.15--100.5) [171]"}
+        (forall e_1: Ref ::
+        { Heap[e_1, q_1] } { QPMask[e_1, q_1] } { refs(Heap, r_1)[e_1] }
+        refs(Heap, r_1)[e_1] && dummyFunction(Heap[e_1, q_1]) ==> wildcard >= NoPerm
+      );
+    
+    // -- check if receiver e is injective
+      assert {:msg "  Folding R(r) might fail. Receiver of e.q [0196.vpr@6.64--6.64]  might not be injective. (0196.vpr@99.15--100.5) [172]"}
+        (forall e_1: Ref, e_1_1: Ref ::
+        { neverTriggered20(e_1), neverTriggered20(e_1_1) }
+        (((e_1 != e_1_1 && refs(Heap, r_1)[e_1]) && refs(Heap, r_1)[e_1_1]) && NoPerm < wildcard) && NoPerm < wildcard ==> e_1 != e_1_1
+      );
+    
+    // -- check if sufficient permission is held
+      assert {:msg "  Folding R(r) might fail. There might be insufficient permission to access e.q (0196.vpr@99.15--100.5) [173]"}
+        (forall e_1: Ref ::
+        { Heap[e_1, q_1] } { QPMask[e_1, q_1] } { refs(Heap, r_1)[e_1] }
+        refs(Heap, r_1)[e_1] ==> Mask[e_1, q_1] > NoPerm
+      );
+    
+    // -- assumptions for inverse of receiver e
+      assume (forall e_1: Ref ::
+        { Heap[e_1, q_1] } { QPMask[e_1, q_1] } { refs(Heap, r_1)[e_1] }
+        refs(Heap, r_1)[e_1] && NoPerm < wildcard ==> qpRange20(e_1) && invRecv20(e_1) == e_1
+      );
+      assume (forall o_2: Ref ::
+        { invRecv20(o_2) }
+        refs(Heap, r_1)[invRecv20(o_2)] && (NoPerm < wildcard && qpRange20(o_2)) ==> invRecv20(o_2) == o_2
+      );
+    
+    // -- assume permission updates for field q
+      assume (forall o_2: Ref ::
+        { QPMask[o_2, q_1] }
+        (refs(Heap, r_1)[invRecv20(o_2)] && (NoPerm < wildcard && qpRange20(o_2)) ==> invRecv20(o_2) == o_2 && QPMask[o_2, q_1] == Mask[o_2, q_1] - wildcard) && (!(refs(Heap, r_1)[invRecv20(o_2)] && (NoPerm < wildcard && qpRange20(o_2))) ==> QPMask[o_2, q_1] == Mask[o_2, q_1])
+      );
+    
+    // -- assume permission updates for independent locations
+      assume (forall <A, B> o_2: Ref, f_4: (Field A B) ::
+        { QPMask[o_2, f_4] }
+        f_4 != q_1 ==> Mask[o_2, f_4] == QPMask[o_2, f_4]
+      );
+    Mask := QPMask;
+    perm := 1 / 2;
+    assume perm >= NoPerm;
+    Mask[null, R(r_1)] := Mask[null, R(r_1)] + perm;
+    assume state(Heap, Mask);
+    assume state(Heap, Mask);
+    assume R#trigger(Heap, R(r_1));
+    assume Heap[null, R(r_1)] == FrameFragment(R#condqp3(Heap, r_1));
+    if (!HasDirectPerm(Mask, null, R(r_1))) {
+      Heap[null, R#sm(r_1)] := ZeroPMask;
+      havoc freshVersion;
+      Heap[null, R(r_1)] := freshVersion;
+    }
+    // register all known folded permissions guarded by predicate R
+    havoc newPMask;
+    assume (forall <A, B> o_5: Ref, f_8: (Field A B) ::
+      { newPMask[o_5, f_8] }
+      Heap[null, R#sm(r_1)][o_5, f_8] ==> newPMask[o_5, f_8]
+    );
+    assume (forall e_2: Ref ::
+      
+      refs(Heap, r_1)[e_2] ==> newPMask[e_2, q_1]
+    );
+    Heap[null, R#sm(r_1)] := newPMask;
+    assume state(Heap, Mask);
+    assume state(Heap, Mask);
+  
+  // -- Translating statement: unfold acc(R(r), 1 / 2) -- 0196.vpr@100.17--101.5
+    assume R#trigger(Heap, R(r_1));
+    assume Heap[null, R(r_1)] == FrameFragment(R#condqp3(Heap, r_1));
+    // Phase 1: pure assertions and fixed permissions
+    assert {:msg "  Unfolding R(r) might fail. Fraction 1 / 2 might be negative. (0196.vpr@100.17--101.5) [174]"}
+      1 / 2 >= NoPerm;
+    perm := NoPerm;
+    perm := perm + 1 / 2;
+    if (perm != NoPerm) {
+      assert {:msg "  Unfolding R(r) might fail. There might be insufficient permission to access R(r) (0196.vpr@100.17--101.5) [175]"}
+        perm <= Mask[null, R(r_1)];
+    }
+    Mask[null, R(r_1)] := Mask[null, R(r_1)] - perm;
+    
+    // -- Update version of predicate
+      if (!HasDirectPerm(Mask, null, R(r_1))) {
+        havoc newVersion;
+        Heap[null, R(r_1)] := newVersion;
+      }
+    assume state(Heap, Mask);
+    havoc QPMask;
+    havoc wildcard;
+    
+    // -- Define Inverse Function
+      assume (forall e_3: Ref ::
+        { Heap[e_3, q_1] } { QPMask[e_3, q_1] } { refs(Heap, r_1)[e_3] }
+        refs(Heap, r_1)[e_3] && NoPerm < wildcard ==> qpRange21(e_3) && invRecv21(e_3) == e_3
+      );
+      assume (forall o_2: Ref ::
+        { invRecv21(o_2) }
+        (refs(Heap, r_1)[invRecv21(o_2)] && NoPerm < wildcard) && qpRange21(o_2) ==> invRecv21(o_2) == o_2
+      );
+    
+    // -- Assume set of fields is nonNull
+      assume (forall e_3: Ref ::
+        { Heap[e_3, q_1] } { QPMask[e_3, q_1] } { refs(Heap, r_1)[e_3] }
+        refs(Heap, r_1)[e_3] && wildcard > NoPerm ==> e_3 != null
+      );
+    // Assume permission expression is non-negative for all fields
+    assume (forall e_3: Ref ::
+      { Heap[e_3, q_1] } { QPMask[e_3, q_1] } { refs(Heap, r_1)[e_3] }
+      refs(Heap, r_1)[e_3] ==> wildcard >= NoPerm
+    );
+    
+    // -- Define permissions
+      assume (forall o_2: Ref ::
+        { QPMask[o_2, q_1] }
+        ((refs(Heap, r_1)[invRecv21(o_2)] && NoPerm < wildcard) && qpRange21(o_2) ==> (NoPerm < wildcard ==> invRecv21(o_2) == o_2) && QPMask[o_2, q_1] == Mask[o_2, q_1] + wildcard) && (!((refs(Heap, r_1)[invRecv21(o_2)] && NoPerm < wildcard) && qpRange21(o_2)) ==> QPMask[o_2, q_1] == Mask[o_2, q_1])
+      );
+      assume (forall <A, B> o_2: Ref, f_4: (Field A B) ::
+        { Mask[o_2, f_4] } { QPMask[o_2, f_4] }
+        f_4 != q_1 ==> Mask[o_2, f_4] == QPMask[o_2, f_4]
+      );
+    Mask := QPMask;
+    assume state(Heap, Mask);
+    assume state(Heap, Mask);
+    assume state(Heap, Mask);
+  
+  // -- Translating statement: r2 := testerfield(get(r)) -- 0196.vpr@101.8--104.1
+    
+    // -- Check definedness of testerfield(get(r))
+      if (*) {
+        // Stop execution
+        assume false;
+      }
+      if (*) {
+        // Exhale precondition of function application
+        // Phase 3: all remaining permissions (containing read permissions, but in a negative context)
+        perm := NoPerm;
+        havoc wildcard;
+        perm := perm + wildcard;
+        assert {:msg "  Precondition of function testerfield might not hold. There might be insufficient permission to access get(r).q (0196.vpr@101.32--101.32) [176]"}
+          Mask[get(Heap, r_1), q_1] > NoPerm;
+        assume wildcard < Mask[get(Heap, r_1), q_1];
+        Mask[get(Heap, r_1), q_1] := Mask[get(Heap, r_1), q_1] - perm;
+        // Finish exhale
+        havoc ExhaleHeap;
+        assume IdenticalOnKnownLocations(Heap, ExhaleHeap, Mask);
+        Heap := ExhaleHeap;
+        // Stop execution
+        assume false;
+      }
+      assume state(Heap, Mask);
+    r2 := testerfield(Heap, get(Heap, r_1));
+    assume state(Heap, Mask);
+}
+
+// ==================================================
+// Translation of method func4
+// ==================================================
+
+procedure func4(r_1: Ref) returns ()
+  modifies Heap, Mask;
+{
+  var perm: Perm;
+  var r2: Ref;
+  var newVersion: FrameType;
+  var wildcard: real where wildcard > NoPerm;
+  var QPMask: MaskType;
+  var freshVersion: FrameType;
+  var newPMask: PMaskType;
+  var ExhaleHeap: HeapType;
+  
+  // -- Initializing the state
+    Mask := ZeroMask;
+    assume state(Heap, Mask);
+    assume AssumeFunctionsAbove == -1;
+  
+  // -- Assumptions about method arguments
+    assume Heap[r_1, $allocated];
+  
+  // -- Checked inhaling of precondition
+    perm := FullPerm;
+    Mask[null, R2(r_1)] := Mask[null, R2(r_1)] + perm;
+    assume state(Heap, Mask);
+    assume state(Heap, Mask);
+  
+  // -- Initializing of old state
+    
+    // -- Initializing the old state
+      assume Heap == old(Heap);
+      assume Mask == old(Mask);
+  
+  // -- Assumptions about local variables
+    assume Heap[r2, $allocated];
+  
+  // -- Translating statement: unfold acc(R2(r), wildcard) -- 0196.vpr@109.18--110.5
+    assume R2#trigger(Heap, R2(r_1));
+    assume Heap[null, R2(r_1)] == FrameFragment(R2#condqp4(Heap, r_1));
+    // Phase 1: pure assertions and fixed permissions
+    
+    // -- Update version of predicate
+      if (!HasDirectPerm(Mask, null, R2(r_1))) {
+        havoc newVersion;
+        Heap[null, R2(r_1)] := newVersion;
+      }
+    // Phase 3: all remaining permissions (containing read permissions, but in a negative context)
+    perm := NoPerm;
+    havoc wildcard;
+    perm := perm + wildcard;
+    assert {:msg "  Unfolding R2(r) might fail. There might be insufficient permission to access R2(r) (0196.vpr@109.18--110.5) [177]"}
+      Mask[null, R2(r_1)] > NoPerm;
+    assume wildcard < Mask[null, R2(r_1)];
+    Mask[null, R2(r_1)] := Mask[null, R2(r_1)] - perm;
+    assume state(Heap, Mask);
+    havoc QPMask;
+    havoc wildcard;
+    
+    // -- Define Inverse Function
+      assume (forall e: Ref ::
+        { Heap[e, q_1] } { QPMask[e, q_1] } { refs(Heap, r_1)[e] }
+        refs(Heap, r_1)[e] && NoPerm < wildcard ==> qpRange22(e) && invRecv22(e) == e
+      );
+      assume (forall o_2: Ref ::
+        { invRecv22(o_2) }
+        (refs(Heap, r_1)[invRecv22(o_2)] && NoPerm < wildcard) && qpRange22(o_2) ==> invRecv22(o_2) == o_2
+      );
+    
+    // -- Assume set of fields is nonNull
+      assume (forall e: Ref ::
+        { Heap[e, q_1] } { QPMask[e, q_1] } { refs(Heap, r_1)[e] }
+        refs(Heap, r_1)[e] && wildcard > NoPerm ==> e != null
+      );
+    // Assume permission expression is non-negative for all fields
+    assume (forall e: Ref ::
+      { Heap[e, q_1] } { QPMask[e, q_1] } { refs(Heap, r_1)[e] }
+      refs(Heap, r_1)[e] ==> wildcard >= NoPerm
+    );
+    
+    // -- Define permissions
+      assume (forall o_2: Ref ::
+        { QPMask[o_2, q_1] }
+        ((refs(Heap, r_1)[invRecv22(o_2)] && NoPerm < wildcard) && qpRange22(o_2) ==> (NoPerm < wildcard ==> invRecv22(o_2) == o_2) && QPMask[o_2, q_1] == Mask[o_2, q_1] + wildcard) && (!((refs(Heap, r_1)[invRecv22(o_2)] && NoPerm < wildcard) && qpRange22(o_2)) ==> QPMask[o_2, q_1] == Mask[o_2, q_1])
+      );
+      assume (forall <A, B> o_2: Ref, f_4: (Field A B) ::
+        { Mask[o_2, f_4] } { QPMask[o_2, f_4] }
+        f_4 != q_1 ==> Mask[o_2, f_4] == QPMask[o_2, f_4]
+      );
+    Mask := QPMask;
+    assume state(Heap, Mask);
+    assume state(Heap, Mask);
+    assume state(Heap, Mask);
+  
+  // -- Translating statement: fold acc(R2(r), wildcard) -- 0196.vpr@110.16--111.5
+    // Phase 1: pure assertions and fixed permissions
+    havoc QPMask;
+    // wild card assumptions
+    havoc wildcard;
+    assert {:msg "  Folding R2(r) might fail. There might be insufficient permission to access e.q (0196.vpr@110.16--111.5) [178]"}
+      (forall e_1: Ref ::
+      
+      refs(Heap, r_1)[e_1] ==> Mask[e_1, q_1] > NoPerm
+    );
+    assume (forall e_1: Ref ::
+      
+      refs(Heap, r_1)[e_1] ==> wildcard < Mask[e_1, q_1]
+    );
+    
+    // -- check that the permission amount is positive
+      assert {:msg "  Folding R2(r) might fail. Fraction 1 / 2 * wildcard might be negative. (0196.vpr@110.16--111.5) [179]"}
+        (forall e_1: Ref ::
+        { Heap[e_1, q_1] } { QPMask[e_1, q_1] } { refs(Heap, r_1)[e_1] }
+        refs(Heap, r_1)[e_1] && dummyFunction(Heap[e_1, q_1]) ==> wildcard >= NoPerm
+      );
+    
+    // -- check if receiver e is injective
+      assert {:msg "  Folding R2(r) might fail. Receiver of e.q [0196.vpr@7.65--7.65]  might not be injective. (0196.vpr@110.16--111.5) [180]"}
+        (forall e_1: Ref, e_1_1: Ref ::
+        { neverTriggered23(e_1), neverTriggered23(e_1_1) }
+        (((e_1 != e_1_1 && refs(Heap, r_1)[e_1]) && refs(Heap, r_1)[e_1_1]) && NoPerm < wildcard) && NoPerm < wildcard ==> e_1 != e_1_1
+      );
+    
+    // -- check if sufficient permission is held
+      assert {:msg "  Folding R2(r) might fail. There might be insufficient permission to access e.q (0196.vpr@110.16--111.5) [181]"}
+        (forall e_1: Ref ::
+        { Heap[e_1, q_1] } { QPMask[e_1, q_1] } { refs(Heap, r_1)[e_1] }
+        refs(Heap, r_1)[e_1] ==> Mask[e_1, q_1] > NoPerm
+      );
+    
+    // -- assumptions for inverse of receiver e
+      assume (forall e_1: Ref ::
+        { Heap[e_1, q_1] } { QPMask[e_1, q_1] } { refs(Heap, r_1)[e_1] }
+        refs(Heap, r_1)[e_1] && NoPerm < wildcard ==> qpRange23(e_1) && invRecv23(e_1) == e_1
+      );
+      assume (forall o_2: Ref ::
+        { invRecv23(o_2) }
+        refs(Heap, r_1)[invRecv23(o_2)] && (NoPerm < wildcard && qpRange23(o_2)) ==> invRecv23(o_2) == o_2
+      );
+    
+    // -- assume permission updates for field q
+      assume (forall o_2: Ref ::
+        { QPMask[o_2, q_1] }
+        (refs(Heap, r_1)[invRecv23(o_2)] && (NoPerm < wildcard && qpRange23(o_2)) ==> invRecv23(o_2) == o_2 && QPMask[o_2, q_1] == Mask[o_2, q_1] - wildcard) && (!(refs(Heap, r_1)[invRecv23(o_2)] && (NoPerm < wildcard && qpRange23(o_2))) ==> QPMask[o_2, q_1] == Mask[o_2, q_1])
+      );
+    
+    // -- assume permission updates for independent locations
+      assume (forall <A, B> o_2: Ref, f_4: (Field A B) ::
+        { QPMask[o_2, f_4] }
+        f_4 != q_1 ==> Mask[o_2, f_4] == QPMask[o_2, f_4]
+      );
+    Mask := QPMask;
+    havoc wildcard;
+    perm := wildcard;
+    Mask[null, R2(r_1)] := Mask[null, R2(r_1)] + perm;
+    assume state(Heap, Mask);
+    assume state(Heap, Mask);
+    assume R2#trigger(Heap, R2(r_1));
+    assume Heap[null, R2(r_1)] == FrameFragment(R2#condqp4(Heap, r_1));
+    if (!HasDirectPerm(Mask, null, R2(r_1))) {
+      Heap[null, R2#sm(r_1)] := ZeroPMask;
+      havoc freshVersion;
+      Heap[null, R2(r_1)] := freshVersion;
+    }
+    // register all known folded permissions guarded by predicate R2
+    havoc newPMask;
+    assume (forall <A, B> o_6: Ref, f_9: (Field A B) ::
+      { newPMask[o_6, f_9] }
+      Heap[null, R2#sm(r_1)][o_6, f_9] ==> newPMask[o_6, f_9]
+    );
+    assume (forall e_2: Ref ::
+      
+      refs(Heap, r_1)[e_2] ==> newPMask[e_2, q_1]
+    );
+    Heap[null, R2#sm(r_1)] := newPMask;
+    assume state(Heap, Mask);
+    assume state(Heap, Mask);
+  
+  // -- Translating statement: unfold acc(R2(r), wildcard) -- 0196.vpr@111.18--112.5
+    assume R2#trigger(Heap, R2(r_1));
+    assume Heap[null, R2(r_1)] == FrameFragment(R2#condqp4(Heap, r_1));
+    // Phase 1: pure assertions and fixed permissions
+    
+    // -- Update version of predicate
+      if (!HasDirectPerm(Mask, null, R2(r_1))) {
+        havoc newVersion;
+        Heap[null, R2(r_1)] := newVersion;
+      }
+    // Phase 3: all remaining permissions (containing read permissions, but in a negative context)
+    perm := NoPerm;
+    havoc wildcard;
+    perm := perm + wildcard;
+    assert {:msg "  Unfolding R2(r) might fail. There might be insufficient permission to access R2(r) (0196.vpr@111.18--112.5) [182]"}
+      Mask[null, R2(r_1)] > NoPerm;
+    assume wildcard < Mask[null, R2(r_1)];
+    Mask[null, R2(r_1)] := Mask[null, R2(r_1)] - perm;
+    assume state(Heap, Mask);
+    havoc QPMask;
+    havoc wildcard;
+    
+    // -- Define Inverse Function
+      assume (forall e_3: Ref ::
+        { Heap[e_3, q_1] } { QPMask[e_3, q_1] } { refs(Heap, r_1)[e_3] }
+        refs(Heap, r_1)[e_3] && NoPerm < wildcard ==> qpRange24(e_3) && invRecv24(e_3) == e_3
+      );
+      assume (forall o_2: Ref ::
+        { invRecv24(o_2) }
+        (refs(Heap, r_1)[invRecv24(o_2)] && NoPerm < wildcard) && qpRange24(o_2) ==> invRecv24(o_2) == o_2
+      );
+    
+    // -- Assume set of fields is nonNull
+      assume (forall e_3: Ref ::
+        { Heap[e_3, q_1] } { QPMask[e_3, q_1] } { refs(Heap, r_1)[e_3] }
+        refs(Heap, r_1)[e_3] && wildcard > NoPerm ==> e_3 != null
+      );
+    // Assume permission expression is non-negative for all fields
+    assume (forall e_3: Ref ::
+      { Heap[e_3, q_1] } { QPMask[e_3, q_1] } { refs(Heap, r_1)[e_3] }
+      refs(Heap, r_1)[e_3] ==> wildcard >= NoPerm
+    );
+    
+    // -- Define permissions
+      assume (forall o_2: Ref ::
+        { QPMask[o_2, q_1] }
+        ((refs(Heap, r_1)[invRecv24(o_2)] && NoPerm < wildcard) && qpRange24(o_2) ==> (NoPerm < wildcard ==> invRecv24(o_2) == o_2) && QPMask[o_2, q_1] == Mask[o_2, q_1] + wildcard) && (!((refs(Heap, r_1)[invRecv24(o_2)] && NoPerm < wildcard) && qpRange24(o_2)) ==> QPMask[o_2, q_1] == Mask[o_2, q_1])
+      );
+      assume (forall <A, B> o_2: Ref, f_4: (Field A B) ::
+        { Mask[o_2, f_4] } { QPMask[o_2, f_4] }
+        f_4 != q_1 ==> Mask[o_2, f_4] == QPMask[o_2, f_4]
+      );
+    Mask := QPMask;
+    assume state(Heap, Mask);
+    assume state(Heap, Mask);
+    assume state(Heap, Mask);
+  
+  // -- Translating statement: r2 := testerfield(get(r)) -- 0196.vpr@112.8--115.1
+    
+    // -- Check definedness of testerfield(get(r))
+      if (*) {
+        // Stop execution
+        assume false;
+      }
+      if (*) {
+        // Exhale precondition of function application
+        // Phase 3: all remaining permissions (containing read permissions, but in a negative context)
+        perm := NoPerm;
+        havoc wildcard;
+        perm := perm + wildcard;
+        assert {:msg "  Precondition of function testerfield might not hold. There might be insufficient permission to access get(r).q (0196.vpr@112.32--112.32) [183]"}
+          Mask[get(Heap, r_1), q_1] > NoPerm;
+        assume wildcard < Mask[get(Heap, r_1), q_1];
+        Mask[get(Heap, r_1), q_1] := Mask[get(Heap, r_1), q_1] - perm;
+        // Finish exhale
+        havoc ExhaleHeap;
+        assume IdenticalOnKnownLocations(Heap, ExhaleHeap, Mask);
+        Heap := ExhaleHeap;
+        // Stop execution
+        assume false;
+      }
+      assume state(Heap, Mask);
+    r2 := testerfield(Heap, get(Heap, r_1));
+    assume state(Heap, Mask);
 }
